[sub] generator begin

part-a.v
@@ -4,7 +4,7 @@
 
    The proofs are written in Coq using de Bruijn indices.
    The whole development took about twelve days.
-*)
+ *)
 
 Set Implicit Arguments.
 Unset Strict Implicit.
@@ -12,14 +12,17 @@ Unset Strict Implicit.
 (* Require Import Arith. *)
 
 From Coq Require Import Lia.
-From Coq Require Import Arith.
-
+From Coq Require Import Arith List String.
+From Coq Require Import Program.Wf.
 From QuickChick Require Import QuickChick.
+From ExtLib Require Import Monad OptionMonad ListMonad.
+Import QcNotation MonadNotation ListNotations.
+
 
 
 (** ** Utils for QuickChick *)
 Instance Dec_eq_opt (A : Type) (m n : option A)
-  `{_ : forall (x y : A), Dec (x = y)} : Dec (m = n).
+         `{_ : forall (x y : A), Dec (x = y)} : Dec (m = n).
 Proof. dec_eq. Defined.
 
 
@@ -32,17 +35,17 @@ Proof. dec_eq. Defined.
 (** ** Standard de Bruijn presentation of Fsub types and terms ***)
 
 Inductive typ : Set :=
-  | tvar : nat -> typ
-  | top : typ
-  | arrow : typ -> typ -> typ
-  | all : typ -> typ -> typ.
+| tvar : nat -> typ
+| top : typ
+| arrow : typ -> typ -> typ
+| all : typ -> typ -> typ.
 
 Inductive term : Set :=
-  | var : nat -> term
-  | abs : typ -> term -> term
-  | app : term -> term -> term
-  | tabs : typ -> term -> term
-  | tapp : term -> typ -> term.
+| var : nat -> term
+| abs : typ -> term -> term
+| app : term -> term -> term
+| tabs : typ -> term -> term
+| tapp : term -> typ -> term.
 
 Instance dec_eq_typ (T1 T2 : typ) : Dec (T1 = T2).
 Proof. dec_eq. Defined.
@@ -124,9 +127,9 @@ Fixpoint subst_typ (t : term) (X : nat) (T : typ) {struct t} : term :=
    [get_var] which access the context. *)
 
 Inductive env : Set :=
-  | empty : env
-  | evar : env -> typ -> env    (* type of var *)
-  | ebound : env -> typ -> env  (* type of tvar *)
+| empty : env
+| evar : env -> typ -> env    (* type of var *)
+| ebound : env -> typ -> env  (* type of tvar *)
 .
 Definition opt_map (A B : Set) (f : A -> B) (x : option A) :=
   match x with
@@ -140,10 +143,10 @@ Fixpoint get_bound (e : env) (X : nat) {struct e} : option typ :=
   | evar e' _ => get_bound e' X
   | ebound e' T =>
       opt_map (tshift 0)
-        (match X with
-         | O    => Some T
-         | S X' => get_bound e' X'
-         end)
+              (match X with
+               | O    => Some T
+               | S X' => get_bound e' X'
+               end)
   end.
 
 Fixpoint get_var (e : env) (x : nat) {struct e} : option typ :=
@@ -156,7 +159,7 @@ Fixpoint get_var (e : env) (x : nat) {struct e} : option typ :=
       | S x' => get_var e' x'
       end
   end.
-          
+
 (****)
 
 (** ** Well-formedness conditions ***)
@@ -267,79 +270,95 @@ Qed.
    We inserted as few well-formedness condition as possible in order
    to reduce the number of time we need to prove that a
    well-formedness condition holds when building a derivation.
-*)
+ *)
 
 Inductive sub : env -> typ -> typ -> Prop :=
-  | SA_Top :
-      forall (e : env) (S : typ), wf_env e -> wf_typ e S -> sub e S top
-  | SA_Refl_TVar :
-      forall (e : env) (X : nat),
-      wf_env e -> wf_typ e (tvar X) -> sub e (tvar X) (tvar X)
-  | SA_Trans_TVar :
-      forall (e : env) (X : nat) (T U : typ),
-      get_bound e X = Some U -> sub e U T -> sub e (tvar X) T
-  | SA_Arrow :
-      forall (e : env) (T1 T2 S1 S2 : typ),
-      sub e T1 S1 -> sub e S2 T2 -> sub e (arrow S1 S2) (arrow T1 T2)
-  | SA_All :
-      forall (e : env) (T1 T2 S1 S2 : typ),
-      sub e T1 S1 -> sub (ebound e T1) S2 T2 -> sub e (all S1 S2) (all T1 T2).
+| SA_Top :
+  forall (e : env) (S : typ), wf_env e -> wf_typ e S -> sub e S top
+| SA_Refl_TVar :
+  forall (e : env) (X : nat),
+    wf_env e -> wf_typ e (tvar X) -> sub e (tvar X) (tvar X)
+| SA_Trans_TVar :
+  forall (e : env) (X : nat) (T U : typ),
+    get_bound e X = Some U -> sub e U T -> sub e (tvar X) T
+| SA_Arrow :
+  forall (e : env) (T1 T2 S1 S2 : typ),
+    sub e T1 S1 -> sub e S2 T2 -> sub e (arrow S1 S2) (arrow T1 T2)
+| SA_All :
+  forall (e : env) (T1 T2 S1 S2 : typ),
+    sub e T1 S1 -> sub (ebound e T1) S2 T2 -> sub e (all S1 S2) (all T1 T2).
 
 
-(* TODO: add [wf_env] and [wf_typ] as premises *)
+(* TODO: add [wf_env] and [wf_typ] as premises, prove [sub_check] terminates *)
 
-Fixpoint typ_measure (T : typ) : nat :=
+Fixpoint measure_typ (T : typ) : nat :=
   match T with
   | tvar _ => 1
   | top => 1
-  | arrow T1 T2 => typ_measure T1 + typ_measure T2 + 1 
-  | all T1 T2 => typ_measure T1 + typ_measure T2 + 1 
+  | arrow T1 T2 => measure_typ T1 + measure_typ T2 + 1 
+  | all T1 T2 => measure_typ T1 + measure_typ T2 + 1 
   end. 
 
-Program Fixpoint sub_check (e : env) (T1 T2 : typ)
-        {measure (measure T1 + measure T2)} : bool :=
-  match T1, T2 with
-  | _, top => true
-  | tvar X1, tvar X2 => X1 = X2 ?
-  | tvar X1, _ =>
-      match get_bound e X1 with
-      | None => false 
-      | Some X1' =>
-          sub_check e X1' T2
+Fixpoint sub_check (e : env) (T1 T2 : typ) (n : nat)
+  : option bool :=
+  match n with
+  | O => None
+  | S n =>  
+      match T1, T2 with
+      | _, top => Some true
+      | tvar X1, tvar X2 => Some (X1 = X2 ?)
+      | tvar X1, _ =>
+          match get_bound e X1 with
+          | None => Some false 
+          | Some X1' =>
+              sub_check e X1' T2 n
+          end
+      | arrow S1 S2, arrow T1 T2 =>
+          match sub_check e T1 S1 n with
+          | Some b1 => match sub_check e S2 T2 n with
+                       | Some b2 => Some (b1 && b2)%bool
+                       | _ => None
+                       end
+          | _ => None
+          end
+      | all S1 S2, all T1 T2 => 
+          match sub_check e T1 S1 n with
+          | Some b1 => match sub_check  (ebound e T1) S2 T2 n with
+                       | Some b2 => Some (b1 && b2)%bool
+                       | _ => None
+                       end
+          | _ => None
+          end
+      | _, _ => Some false
       end
-  | arrow S1 S2, arrow T1 T2 =>
-      sub_check e T1 S1 && sub_check e S2 T2
-  | all S1 S2, all T1 T2 =>
-      sub_check e T1 S1 && sub_check (ebound e T1) S2 T2
-  | _, _ => false
-  end
-.
+  end.
+
 (****)
 
 (** ** Typing relation ***)
 
 Inductive typing : env -> term -> typ -> Prop :=
-  | T_Var :
-      forall (e : env) (x : nat) (T : typ),
-      wf_env e -> get_var e x = Some T -> typing e (var x) T
-  | T_Abs :
-      forall (e : env) (t : term) (T1 T2 : typ),
-      typing (evar e T1) t T2 ->
-      typing e (abs T1 t) (arrow T1 T2)
-  | T_App :
-      forall (e : env) (t1 t2 : term) (T11 T12 : typ),
-      typing e t1 (arrow T11 T12) ->
-      typing e t2 T11 -> typing e (app t1 t2) T12
-  | T_Tabs :
-      forall (e : env) (t : term) (T1 T2 : typ),
-      typing (ebound e T1) t T2 -> typing e (tabs T1 t) (all T1 T2)
-  | T_Tapp :
-      forall (e : env) (t1 : term) (T11 T12 T2 : typ),
-      typing e t1 (all T11 T12) ->
-      sub e T2 T11 -> typing e (tapp t1 T2) (tsubst T12 0 T2)
-  | T_Sub :
-      forall (e : env) (t : term) (T1 T2 : typ),
-      typing e t T1 -> sub e T1 T2 -> typing e t T2.
+| T_Var :
+  forall (e : env) (x : nat) (T : typ),
+    wf_env e -> get_var e x = Some T -> typing e (var x) T
+| T_Abs :
+  forall (e : env) (t : term) (T1 T2 : typ),
+    typing (evar e T1) t T2 ->
+    typing e (abs T1 t) (arrow T1 T2)
+| T_App :
+  forall (e : env) (t1 t2 : term) (T11 T12 : typ),
+    typing e t1 (arrow T11 T12) ->
+    typing e t2 T11 -> typing e (app t1 t2) T12
+| T_Tabs :
+  forall (e : env) (t : term) (T1 T2 : typ),
+    typing (ebound e T1) t T2 -> typing e (tabs T1 t) (all T1 T2)
+| T_Tapp :
+  forall (e : env) (t1 : term) (T11 T12 T2 : typ),
+    typing e t1 (all T11 T12) ->
+    sub e T2 T11 -> typing e (tapp t1 T2) (tsubst T12 0 T2)
+| T_Sub :
+  forall (e : env) (t : term) (T1 T2 : typ),
+    typing e t T1 -> sub e T1 T2 -> typing e t T2.
 
 
 Fixpoint get_typ (e : env) (t : term) : option typ :=
@@ -369,27 +388,25 @@ Fixpoint get_typ (e : env) (t : term) : option typ :=
   | tapp t1 T2 => 
       match get_typ e t1 with
       | Some (all T11 T12) =>
-          
+          match sub_check e T2 T11 (measure_typ T2 + measure_typ T11) with
+          | Some true => Some (tsubst T12 0 T2)
+          | _ => None
+          end
       | _ => None
       end
-      
-
-Fixpoint type_check (e : env) (t : term) (T : typ) : bool :=
-  match t with
-  | var x =>
-      dc_wf_env e &&
-        match get_var e x with
-        | None => false
-        | Some T' => T = T' ?
-        end
-  | abs T1 t2 =>
-      type_check (evar e T1)  t2
-  | app t1 t2 =>
-      
-  | _ => false
   end.
 
-                                      
+
+Definition type_check (e : env) (t : term) (T : typ) : bool :=
+  match get_typ e t with
+  | Some T' =>
+      match sub_check e T' T (measure_typ T' + measure_typ T) with
+      | Some true => true
+      | _ => false
+      end
+  | None => false
+  end.
+
 (****)
 
 (** ** Reduction rules ***)
@@ -401,11 +418,21 @@ Definition value (t : term) :=
   | _        => False
   end.
 
+Definition dc_value (t : term) : bool :=
+  match t with
+  | abs _ _  => true
+  | tabs _ _ => true
+  | _        => false
+  end.
+
+Lemma dc_value_implies_value : forall t, dc_value t = true -> value t.
+Proof. intros t. destruct t; cbn; auto. Qed.
+
 Inductive ctx : Type :=
-    c_hole : ctx
-  | c_appfun : ctx -> term -> ctx
-  | c_apparg : forall (t : term), value t -> ctx -> ctx
-  | c_typefun : ctx -> typ -> ctx.
+  c_hole : ctx
+| c_appfun : ctx -> term -> ctx
+| c_apparg : forall (t : term), value t -> ctx -> ctx
+| c_typefun : ctx -> typ -> ctx.
 
 Fixpoint ctx_app (c : ctx) (t : term) {struct c} : term :=
   match c with
@@ -417,26 +444,90 @@ Fixpoint ctx_app (c : ctx) (t : term) {struct c} : term :=
 
 
 Inductive red : term -> term -> Prop :=
-  | E_AppAbs :
-      forall (t11 : typ) (t12 t2 : term),
-      value t2 -> red (app (abs t11 t12) t2) (subst t12 0 t2)
-  | E_TappTabs :
-      forall (t11 t2 : typ) (t12 : term),
-      red (tapp (tabs t11 t12) t2) (subst_typ t12 0 t2)
-  | E_Ctx :
-      forall (c : ctx) (t1 t1' : term),
-      red t1 t1' -> red (ctx_app c t1) (ctx_app c t1').
+| E_AppAbs :
+  forall (t11 : typ) (t12 t2 : term),
+    value t2 -> red (app (abs t11 t12) t2) (subst t12 0 t2)
+| E_TappTabs :
+  forall (t11 t2 : typ) (t12 : term),
+    red (tapp (tabs t11 t12) t2) (subst_typ t12 0 t2)
+| E_Ctx :
+  forall (c : ctx) (t1 t1' : term),
+    red t1 t1' -> red (ctx_app c t1) (ctx_app c t1').
 
+
+(** reduction semantics per step  *)
+
+Program Definition ctx_inj (t : term) : option (ctx * term) :=
+  match t with
+  | app t1 t2 =>
+      match dc_value t1 with
+        true => Some (@c_apparg t1 _ c_hole, t2)
+      | false => Some (c_appfun c_hole t2, t1)
+      end
+  | tapp t1 T2 =>
+      Some (c_typefun c_hole T2,  t1)
+  | _ => None
+  end.
+Next Obligation.
+  apply dc_value_implies_value. auto.
+Qed.
+Solve All Obligations with easy.
+
+Eval cbn in (ctx_inj (tapp (var 0) top)).
+
+
+Fixpoint measure_term (t : term) : nat :=
+  match t with
+  | var _ => 1 
+  | abs _ t' => 1 + measure_term t'
+  | app t1 t2 => 1 + measure_term t1 + measure_term t2
+  | tabs _ t2 => 1 + measure_term t2
+  | tapp t1 _ => 1 + measure_term t1
+  end.
+
+Lemma measure_term_le_ctx_inj : forall c t t',
+    Some (c, t') = ctx_inj t -> measure_term t' < measure_term t.
+Proof.
+  intros until t. destruct t; intros; cbn in *; try congruence. 
+  - destruct t1; cbn in *; inversion H; clear H; subst; cbn; lia.
+  - inversion H; clear H; subst; lia. 
+Qed.
+
+Program Fixpoint step (t : term) {measure (measure_term t) lt} : option term :=
+  match t with
+  | app (abs _ t12) t2 =>
+      if dc_value t2 then Some (subst t12 0 t2) else
+        match ctx_inj t with
+        | None => None
+        | Some (c', t') => 
+            match step t' with
+            | Some t'' => Some (ctx_app c' t'')
+            | None => None
+            end
+        end         
+  | tapp (tabs T11 t12) T2 => Some (subst_typ t12 0 T2)
+  | _ => match ctx_inj t with
+         | None => None
+         | Some (c', t') => 
+             match step t' with
+             | Some t'' => Some (ctx_app c' t'')
+             | None => None
+             end
+         end 
+  end.
+
+Next Obligation.
+  cbn; lia.
+Qed.
+Next Obligation.
+  apply (measure_term_le_ctx_inj Heq_anonymous).
+Qed.
+Solve All Obligations with easy.
 
 (*************************************************************************)
 (*                            General lemmas                             *)
 (*************************************************************************)
-
-
 (** ** Commutation properties of shifting and substitution ***)
-
-Check lt_eq_lt_dec.
-
 
 Ltac tvar_case :=
   unfold tshift; unfold tsubst; fold tshift; fold tsubst;
@@ -452,49 +543,49 @@ Ltac tvar_case :=
 
 Ltac common_cases n T :=
   simpl; generalize n; clear n; induction T; intros n''; intros;
-    [ repeat tvar_case;
-      simpl; trivial; try (intros; apply f_equal with (f := tvar); lia);
-      try (intros; assert False; [ lia | contradiction ])
-    | trivial
-    | simpl; apply f_equal2 with (f := arrow); trivial
-    | simpl; apply f_equal2 with (f := all); trivial ].
+  [ repeat tvar_case;
+    simpl; trivial; try (intros; apply f_equal with (f := tvar); lia);
+    try (intros; assert False; [ lia | contradiction ])
+  | trivial
+  | simpl; apply f_equal2 with (f := arrow); trivial
+  | simpl; apply f_equal2 with (f := all); trivial ].
 
 Lemma tsubst_tshift_prop :
   forall (n : nat) (T T' : typ), T = tsubst (tshift n T) n T'.
-intros n T; common_cases n T.
+  intros n T; common_cases n T.
 Qed.
 
 Lemma tshift_tshift_prop_1 :
   forall (n n' : nat) (T : typ),
-  tshift n (tshift (n + n') T) = tshift (1 + (n + n')) (tshift n T).
-intros n n' T; common_cases n T; exact (IHT2 (S n'')).
+    tshift n (tshift (n + n') T) = tshift (1 + (n + n')) (tshift n T).
+  intros n n' T; common_cases n T; exact (IHT2 (S n'')).
 Qed.
 
 Lemma tshift_tsubst_prop_1 :
   forall (n n' : nat) (T T' : typ),
-  tshift n (tsubst T (n + n') T') =
-  tsubst (tshift n T) (1 + n + n') (tshift n T').
-intros n n' T; common_cases n T;
-rewrite (tshift_tshift_prop_1 0 n''); apply (IHT2 (S n'')).
+    tshift n (tsubst T (n + n') T') =
+      tsubst (tshift n T) (1 + n + n') (tshift n T').
+  intros n n' T; common_cases n T;
+    rewrite (tshift_tshift_prop_1 0 n''); apply (IHT2 (S n'')).
 Qed.
 
 Lemma tshift_tsubst_prop_2 :
   forall (n n' : nat) (T T' : typ),
-  (tshift (n + n') (tsubst T n T')) =
-  (tsubst (tshift (1 + n + n') T) n (tshift (n + n') T')).
-intros n n' T; common_cases n T;
-rewrite (tshift_tshift_prop_1 0 (n'' + n')); apply (IHT2 (S n'')).
+    (tshift (n + n') (tsubst T n T')) =
+      (tsubst (tshift (1 + n + n') T) n (tshift (n + n') T')).
+  intros n n' T; common_cases n T;
+    rewrite (tshift_tshift_prop_1 0 (n'' + n')); apply (IHT2 (S n'')).
 Qed.
 
 Lemma tsubst_tsubst_prop :
   forall (n n' : nat) (T U V : typ),
-  (tsubst (tsubst T n U) (n + n') V) =
-  (tsubst (tsubst T (1 + n + n') (tshift n V)) n (tsubst U (n + n') V)).
-intros n n' T; common_cases n T;
-  [ intros; apply tsubst_tshift_prop
-  | rewrite (tshift_tsubst_prop_1 0 (n'' + n'));
-    rewrite (tshift_tshift_prop_1 0 n'');
-    apply (IHT2 (S n'')) ].
+    (tsubst (tsubst T n U) (n + n') V) =
+      (tsubst (tsubst T (1 + n + n') (tshift n V)) n (tsubst U (n + n') V)).
+  intros n n' T; common_cases n T;
+    [ intros; apply tsubst_tshift_prop
+    | rewrite (tshift_tsubst_prop_1 0 (n'' + n'));
+      rewrite (tshift_tshift_prop_1 0 n'');
+      apply (IHT2 (S n'')) ].
 Qed.
 
 (****)
@@ -503,13 +594,13 @@ Qed.
 
 Lemma wf_typ_env_weaken :
   forall (T : typ) (e e' : env),
-  (forall (X : nat), get_bound e' X = None -> get_bound e X = None) ->
-  wf_typ e T -> wf_typ e' T.
-induction T; simpl; auto; intros e e' H (H1, H2); split;
-  [ apply (IHT1 _ _ H H1)
-  | apply (IHT2 _ _ H H2)
-  | apply (IHT1 _ _ H H1)
-  | apply IHT2 with (2 := H2); induction X;
+    (forall (X : nat), get_bound e' X = None -> get_bound e X = None) ->
+    wf_typ e T -> wf_typ e' T.
+  induction T; simpl; auto; intros e e' H (H1, H2); split;
+    [ apply (IHT1 _ _ H H1)
+    | apply (IHT2 _ _ H H2)
+    | apply (IHT1 _ _ H H1)
+    | apply IHT2 with (2 := H2); induction X;
       [ trivial
       | simpl; intro H3; rewrite H; trivial;
         generalize H3; case (get_bound e' X); simpl; trivial;
@@ -518,10 +609,10 @@ Qed.
 
 Lemma wf_typ_extensionality :
   forall (T : typ) (e e' : env),
-  (forall (X : nat), get_bound e X = get_bound e' X) ->
-  wf_typ e T -> wf_typ e' T.
-intros T e e' H1 H2; apply wf_typ_env_weaken with (2 := H2);
-intros n H3; rewrite H1; trivial.
+    (forall (X : nat), get_bound e X = get_bound e' X) ->
+    wf_typ e T -> wf_typ e' T.
+  intros T e e' H1 H2; apply wf_typ_env_weaken with (2 := H2);
+    intros n H3; rewrite H1; trivial.
 Qed.
 
 (****)
@@ -531,7 +622,7 @@ Qed.
 (*
    This corresponds to the environment operation
       E, x : T, E'  |-->  E.
-*)
+ *)
 
 Fixpoint remove_var (e : env) (x : nat) {struct e} : env :=
   match e with
@@ -546,54 +637,54 @@ Fixpoint remove_var (e : env) (x : nat) {struct e} : env :=
 
 Lemma get_var_remove_var_lt :
   forall (e : env) (x x' : nat),
-  x < x' -> get_var (remove_var e x') x = get_var e x.
-induction e; simpl; trivial; intros n n' H;
-  [ induction n';
+    x < x' -> get_var (remove_var e x') x = get_var e x.
+  induction e; simpl; trivial; intros n n' H;
+    [ induction n';
       [ inversion H
       | clear IHn'; induction n; simpl; trivial;
         apply IHe; lia ]
-  | apply f_equal with (f := opt_map (tshift 0)); auto ].
+    | apply f_equal with (f := opt_map (tshift 0)); auto ].
 Qed.
 
 Lemma get_var_remove_var_ge :
   forall (e : env) (x x' : nat),
-  x >= x' -> get_var (remove_var e x') x = get_var e (1 + x).
-induction e; simpl; trivial; intros n n' H;
-  [ induction n'; trivial;
-    clear IHn'; induction n;
+    x >= x' -> get_var (remove_var e x') x = get_var e (1 + x).
+  induction e; simpl; trivial; intros n n' H;
+    [ induction n'; trivial;
+      clear IHn'; induction n;
       [ inversion H
       | simpl; apply (IHe n); lia ]
-  | apply f_equal with (f := opt_map (tshift 0)); apply (IHe n); trivial ].
+    | apply f_equal with (f := opt_map (tshift 0)); apply (IHe n); trivial ].
 Qed.
 
 Lemma get_bound_remove_var :
   forall (e : env) (X x': nat), get_bound e X = get_bound (remove_var e x') X.
-induction e; simpl; trivial; intros n n';
-  [ induction n'; simpl; trivial
-  | induction n; trivial;
-    apply f_equal with (f := opt_map (tshift 0)); trivial ].
+  induction e; simpl; trivial; intros n n';
+    [ induction n'; simpl; trivial
+    | induction n; trivial;
+      apply f_equal with (f := opt_map (tshift 0)); trivial ].
 Qed.
 
 Lemma wf_typ_remove_var :
   forall (e : env) (x : nat) (T : typ),
-  wf_typ e T -> wf_typ (remove_var e x) T.
-intros e n T; apply wf_typ_extensionality;
-intro n'; apply get_bound_remove_var.
+    wf_typ e T -> wf_typ (remove_var e x) T.
+  intros e n T; apply wf_typ_extensionality;
+    intro n'; apply get_bound_remove_var.
 Qed.
 
 Lemma wf_typ_insert_var :
   forall (e : env) (n : nat) (T : typ),
-  wf_typ (remove_var e n) T -> wf_typ e T.
-intros e n T; apply wf_typ_extensionality; intro n';
-apply sym_eq; apply get_bound_remove_var.
+    wf_typ (remove_var e n) T -> wf_typ e T.
+  intros e n T; apply wf_typ_extensionality; intro n';
+    apply sym_eq; apply get_bound_remove_var.
 Qed.
 
 Lemma wf_env_remove_var :
   forall (e : env) (x : nat), wf_env e -> wf_env (remove_var e x).
-induction e; simpl; trivial;
-  [ intros n (H1, H2); induction n; trivial;
-    simpl; split; auto; apply wf_typ_remove_var; trivial
-  | intros n (H1, H2); split; auto; apply wf_typ_remove_var; trivial ].
+  induction e; simpl; trivial;
+    [ intros n (H1, H2); induction n; trivial;
+      simpl; split; auto; apply wf_typ_remove_var; trivial
+    | intros n (H1, H2); split; auto; apply wf_typ_remove_var; trivial ].
 Qed.
 
 (****)
@@ -604,40 +695,40 @@ Qed.
    This corresponds to the environment operation
        E, E'  |-->  E, X <: T, E'.
    Note that all type variable in E' has to be shifted.
-*)
+ *)
 
 Inductive insert_bound : nat -> env -> env -> Prop :=
-    ib_here :
-      forall (T : typ) (e : env), wf_typ e T -> insert_bound 0 e (ebound e T)
-  | ib_var :
-      forall (X : nat) (T : typ) (e e' : env),
-      insert_bound X e e' ->
-      insert_bound X (evar e T) (evar e' (tshift X T))
-  | ib_bound :
-      forall (X : nat) (T : typ) (e e' : env),
-      insert_bound X e e' ->
-      insert_bound (1 + X) (ebound e T) (ebound e' (tshift X T)).
+  ib_here :
+    forall (T : typ) (e : env), wf_typ e T -> insert_bound 0 e (ebound e T)
+| ib_var :
+  forall (X : nat) (T : typ) (e e' : env),
+    insert_bound X e e' ->
+    insert_bound X (evar e T) (evar e' (tshift X T))
+| ib_bound :
+  forall (X : nat) (T : typ) (e e' : env),
+    insert_bound X e e' ->
+    insert_bound (1 + X) (ebound e T) (ebound e' (tshift X T)).
 
 Lemma get_bound_insert_bound_ge :
   forall (X X' : nat) (e e' : env),
-  insert_bound X' e e' -> X' <= X ->
-  get_bound e' (1 + X) = opt_map (tshift X') (get_bound e X).
-simpl; intros n n' e e' H; generalize n; clear n; induction H; simpl; trivial;
-intros n' H1; induction n'; simpl;
-  [ inversion H1
-  | clear IHn'; rewrite IHinsert_bound; try lia;
-    case (get_bound e n'); simpl; trivial;
-    intro T''; apply f_equal with (f := @Some typ);
-    apply (tshift_tshift_prop_1 0 X) ].
+    insert_bound X' e e' -> X' <= X ->
+    get_bound e' (1 + X) = opt_map (tshift X') (get_bound e X).
+  simpl; intros n n' e e' H; generalize n; clear n; induction H; simpl; trivial;
+    intros n' H1; induction n'; simpl;
+    [ inversion H1
+    | clear IHn'; rewrite IHinsert_bound; try lia;
+      case (get_bound e n'); simpl; trivial;
+      intro T''; apply f_equal with (f := @Some typ);
+      apply (tshift_tshift_prop_1 0 X) ].
 Qed.
 
 Lemma get_bound_insert_bound_lt :
   forall (X X' : nat) (e e' : env),
-  insert_bound X' e e' -> X < X' ->
-  get_bound e' X = opt_map (tshift X') (get_bound e X).
-intros n n' e e' H; generalize n; clear n; induction H; simpl; trivial;
-  [ intros n H1; inversion H1
-  | intros n' H1; induction n';
+    insert_bound X' e e' -> X < X' ->
+    get_bound e' X = opt_map (tshift X') (get_bound e X).
+  intros n n' e e' H; generalize n; clear n; induction H; simpl; trivial;
+    [ intros n H1; inversion H1
+    | intros n' H1; induction n';
       [ simpl; apply f_equal with (f := @Some typ);
         apply (tshift_tshift_prop_1 0 X)
       | clear IHn'; rewrite IHinsert_bound; try lia;
@@ -648,27 +739,27 @@ Qed.
 
 Lemma get_var_insert_bound :
   forall (x X' : nat) (e e' : env),
-  insert_bound X' e e' -> get_var e' x = opt_map (tshift X') (get_var e x).
-intros n n' e e' H; generalize n; clear n; induction H; simpl; intro n';
-  [ trivial
-  | induction n'; trivial
-  | rewrite IHinsert_bound; case (get_var e n'); simpl; trivial;
-    intro T'; apply f_equal with (f := @Some typ);
-    apply (tshift_tshift_prop_1 0 X) ].
+    insert_bound X' e e' -> get_var e' x = opt_map (tshift X') (get_var e x).
+  intros n n' e e' H; generalize n; clear n; induction H; simpl; intro n';
+    [ trivial
+    | induction n'; trivial
+    | rewrite IHinsert_bound; case (get_var e n'); simpl; trivial;
+      intro T'; apply f_equal with (f := @Some typ);
+      apply (tshift_tshift_prop_1 0 X) ].
 Qed.
 
 Lemma insert_bound_wf_typ :
   forall (T : typ) (X : nat) (e e' : env),
-  insert_bound X e e' -> wf_typ e T -> wf_typ e' (tshift X T).
-induction T;
-  [ unfold tshift; fold tshift; intros n' e e' H1 H2; case (le_gt_dec n' n);
+    insert_bound X e e' -> wf_typ e T -> wf_typ e' (tshift X T).
+  induction T;
+    [ unfold tshift; fold tshift; intros n' e e' H1 H2; case (le_gt_dec n' n);
       [ intro H3; unfold wf_typ; rewrite (get_bound_insert_bound_ge H1 H3);
         intro H4; apply H2; induction (get_bound e n); trivial; discriminate
       | intro H3; simpl; rewrite (get_bound_insert_bound_lt H1 H3);
         intro H4; apply H2; induction (get_bound e n); trivial; discriminate ]
-  | trivial
-  | simpl; intros n e e' H1 (H2, H3); eauto
-  | simpl; intros n e e' H1 (H2, H3); split;
+    | trivial
+    | simpl; intros n e e' H1 (H2, H3); eauto
+    | simpl; intros n e e' H1 (H2, H3); split;
       [ apply (IHT1 _ _ _ H1 H2)
       | apply IHT2 with (e := (ebound e T1)); trivial;
         exact (ib_bound T1 H1) ] ].
@@ -676,9 +767,9 @@ Qed.
 
 Lemma insert_bound_wf_env :
   forall (X : nat) (e e' : env),
-  insert_bound X e e' -> wf_env e -> wf_env e'.
-intros n e e' H; induction H; simpl; auto;
-intros (H1, H2); split; auto; exact (insert_bound_wf_typ H H1).
+    insert_bound X e e' -> wf_env e -> wf_env e'.
+  intros n e e' H; induction H; simpl; auto;
+    intros (H1, H2); split; auto; exact (insert_bound_wf_typ H H1).
 Qed.
 
 (****)
@@ -687,49 +778,76 @@ Qed.
 
 Lemma wf_typ_weakening_bound :
   forall (e : env) (T U : typ),
-  wf_typ e T -> wf_typ e U -> wf_typ (ebound e U) (tshift 0 T).
-intros e T U H1 H2; apply insert_bound_wf_typ with (2 := H1);
-apply ib_here; trivial.
+    wf_typ e T -> wf_typ e U -> wf_typ (ebound e U) (tshift 0 T).
+  intros e T U H1 H2; apply insert_bound_wf_typ with (2 := H1);
+    apply ib_here; trivial.
 Qed.
 
 Lemma wf_typ_weakening_var :
   forall (e : env) (T U : typ),
-  wf_typ e U -> wf_typ (evar e T) U.
-intros e T U H; apply wf_typ_env_weaken with (2 := H); simpl; trivial.
+    wf_typ e U -> wf_typ (evar e T) U.
+  intros e T U H; apply wf_typ_env_weaken with (2 := H); simpl; trivial.
 Qed.
 
 Lemma wf_typ_strengthening_var :
   forall (e : env) (T U : typ),
-  wf_typ (evar e T) U -> wf_typ e U.
-intros e T U H; apply wf_typ_env_weaken with (2 := H); simpl; trivial.
+    wf_typ (evar e T) U -> wf_typ e U.
+  intros e T U H; apply wf_typ_env_weaken with (2 := H); simpl; trivial.
 Qed.
 
 Lemma wf_typ_ebound :
   forall (T U V : typ) (e : env),
-  wf_typ (ebound e U) T -> wf_typ (ebound e V) T.
-intros T U V e; apply wf_typ_env_weaken; intro X; induction X;
-  [ intros; discriminate
-  | trivial ].
+    wf_typ (ebound e U) T -> wf_typ (ebound e V) T.
+  intros T U V e; apply wf_typ_env_weaken; intro X; induction X;
+    [ intros; discriminate
+    | trivial ].
 Qed.
 
 Lemma get_var_wf :
   forall (e : env) (n : nat) (T : typ),
-  wf_env e -> get_var e n = Some T -> wf_typ e T.
-induction e; simpl;
-  [ intros; discriminate
-  | induction n; intros T (H1, H2) E;
+    wf_env e -> get_var e n = Some T -> wf_typ e T.
+  induction e; simpl;
+    [ intros; discriminate
+    | induction n; intros T (H1, H2) E;
       [ injection E; clear E; intro E;
         rewrite <- E; exact (wf_typ_weakening_var t H1)
       | apply wf_typ_weakening_var; eauto ]
-  | intros n T (H1, H2) E; assert (H3 := IHe n); clear IHe;
-    induction (get_var e n);
+    | intros n T (H1, H2) E; assert (H3 := IHe n); clear IHe;
+      induction (get_var e n);
       [ simpl in E; injection E; clear E; intro E; rewrite <- E;
         apply wf_typ_weakening_bound with (2 := H1); apply H3 with (1 := H2);
         trivial
       | discriminate ] ].
 Qed.
 
+Fixpoint count_var (E : env) : nat :=
+  match E with
+  | empty => 0
+  | evar E _ => S (count_var E)
+  | ebound E _ => (count_var E)
+  end.
 
+Check returnGen .
+
+Definition gen_typ_from_env (E : env) : G (option typ) :=
+  match count_var E with
+  | O => ret None
+  | S n => n' <- choose(0, n);; ret (get_var E n')
+  end.
+
+(** ** Type Generator *)
+Fixpoint gen_typ (fuel : nat) (E : env) : G typ :=
+  match fuel with
+  | O =>
+      oT <- gen_typ_from_env E;;
+      match oT with
+      | None => ret top
+      | Some T => elems [top ; T]
+      end
+  | S n =>
+      ret top
+  end.
+      
 (*************************************************************************)
 (*                       Transitivity of subtyping                       *)
 (*************************************************************************)
@@ -739,11 +857,21 @@ Qed.
 
 Lemma sub_wf :
   forall (e : env) (T U : typ),
-  sub e T U -> wf_env e /\ wf_typ e T /\ wf_typ e U.
-intros e T U H; induction H; repeat split; simpl; trivial; try tauto;
-  [ rewrite H; discriminate
-  | apply wf_typ_ebound with (U := T1); tauto ].
+    sub e T U -> wf_env e /\ wf_typ e T /\ wf_typ e U.
+  intros e T U H; induction H; repeat split; simpl; trivial; try tauto;
+    [ rewrite H; discriminate
+    | apply wf_typ_ebound with (U := T1); tauto ].
 Qed.
+
+Definition prop_gen_wt :=
+  let fuel_type := 4 in
+  let fuel_expr := 4 in
+  forAll (gen_type fuel_type) (fun T =>
+  forAllMaybe (gen_expr fuel_expr [] T) (fun t => 
+  whenFail ("Type was " ++ show T ++ nl ++ 
+            "Term was " ++ show t ++ nl ++
+            "With Type" ++ show (typeOf [] t) ++))
+           (typeOf [] t = Some T ?)).
 
 (****)
 
@@ -751,16 +879,18 @@ Qed.
 
 Lemma sub_reflexivity :
   forall (e : env) (T : typ), wf_env e -> wf_typ e T -> sub e T T.
-intros e T; generalize e; clear e; induction T; intros e H1 H2;
-  [ apply SA_Refl_TVar; trivial
-  | apply SA_Top; trivial
-  | apply SA_Arrow;
+  intros e T; generalize e; clear e; induction T; intros e H1 H2;
+    [ apply SA_Refl_TVar; trivial
+    | apply SA_Top; trivial
+    | apply SA_Arrow;
       [ exact (IHT1 _ H1 (proj1 H2))
       | exact (IHT2 _ H1 (proj2 H2)) ]
-  | apply SA_All;
+    | apply SA_All;
       [ exact (IHT1 _ H1 (proj1 H2))
       | apply IHT2 with (2 := (proj2 H2)); simpl; simpl in H2; tauto ] ].
 Qed.
+
+
 
 (****)
 
@@ -773,36 +903,36 @@ Qed.
    the environment.
    The shifting is needed as a type variable binding is inserted in
    the environment.
-*)
+ *)
 
 Lemma sub_weakening_bound_ind :
   forall (e e' : env) (X : nat) (U V : typ),
-  insert_bound X e e' -> sub e U V -> sub e' (tshift X U) (tshift X V).
-intros e e' X U V H1 H2; generalize X e' H1; clear X e' H1;
-induction H2; intros X' e' H1; simpl;
-  [ apply SA_Top;
+    insert_bound X e e' -> sub e U V -> sub e' (tshift X U) (tshift X V).
+  intros e e' X U V H1 H2; generalize X e' H1; clear X e' H1;
+    induction H2; intros X' e' H1; simpl;
+    [ apply SA_Top;
       [ exact (insert_bound_wf_env H1 H)
       | exact (insert_bound_wf_typ H1 H0) ]
-  | apply SA_Refl_TVar;
+    | apply SA_Refl_TVar;
       [ exact (insert_bound_wf_env H1 H)
       | exact (insert_bound_wf_typ H1 H0) ]
-  | apply SA_Trans_TVar with (2 := (IHsub X' e' H1));
-    case (le_gt_dec X' X); intro H3;
+    | apply SA_Trans_TVar with (2 := (IHsub X' e' H1));
+      case (le_gt_dec X' X); intro H3;
       [ change (S X) with (1 + X); trivial;
         rewrite get_bound_insert_bound_ge with (1 := H1) (2 := H3);
         rewrite H; trivial
       | rewrite get_bound_insert_bound_lt with (1 := H1) (2 := H3);
         rewrite H; trivial ]
-  | apply SA_Arrow; auto
-  | apply SA_All; auto;
-    exact (IHsub2 (1 + X') _ (ib_bound T1 H1)) ].
+    | apply SA_Arrow; auto
+    | apply SA_All; auto;
+      exact (IHsub2 (1 + X') _ (ib_bound T1 H1)) ].
 Qed.
 
 Lemma sub_weakening_bound :
   forall (e : env) (T U V : typ),
-  wf_typ e V -> sub e T U -> sub (ebound e V) (tshift 0 T) (tshift 0 U).
-intros e T U V H0 H; apply sub_weakening_bound_ind with (2 := H);
-apply ib_here; trivial.
+    wf_typ e V -> sub e T U -> sub (ebound e V) (tshift 0 T) (tshift 0 U).
+  intros e T U V H0 H; apply sub_weakening_bound_ind with (2 := H);
+    apply ib_here; trivial.
 Qed.
 
 (*
@@ -811,20 +941,20 @@ Qed.
    paper proof), we prove the more general result that the subtyping
    relation does not depend on the term variable bindings.  Then, this
    intermediate result can be used for proving strengthening.
-*)
+ *)
 
 Lemma sub_extensionality :
   forall (e e' : env) (U V : typ),
-  (forall (X : nat), (get_bound e X) = (get_bound e' X)) -> wf_env e' ->
-  sub e U V -> sub e' U V.
-intros e e' U V H0 H1 H2; generalize e' H0 H1; clear e' H0 H1;
-induction H2; intros e' H3 H1;
-  [ apply SA_Top; trivial; exact (wf_typ_extensionality H3 H0)
-  | apply SA_Refl_TVar; trivial; exact (wf_typ_extensionality H3 H0)
-  | rewrite H3 in H; apply SA_Trans_TVar with (1 := H); auto
-  | apply SA_Arrow; auto
-  | apply SA_All; auto;
-    apply IHsub2 with (e' := (ebound e' T1));
+    (forall (X : nat), (get_bound e X) = (get_bound e' X)) -> wf_env e' ->
+    sub e U V -> sub e' U V.
+  intros e e' U V H0 H1 H2; generalize e' H0 H1; clear e' H0 H1;
+    induction H2; intros e' H3 H1;
+    [ apply SA_Top; trivial; exact (wf_typ_extensionality H3 H0)
+    | apply SA_Refl_TVar; trivial; exact (wf_typ_extensionality H3 H0)
+    | rewrite H3 in H; apply SA_Trans_TVar with (1 := H); auto
+    | apply SA_Arrow; auto
+    | apply SA_All; auto;
+      apply IHsub2 with (e' := (ebound e' T1));
       [ intro X; induction X; simpl; trivial; rewrite H3; trivial
       | simpl; split; trivial;
         apply wf_typ_extensionality with (1 := H3);
@@ -833,16 +963,16 @@ Qed.
 
 Lemma sub_weakening_var_ind :
   forall (e : env) (x : nat) (U V : typ),
-  wf_env e -> sub (remove_var e x) U V -> sub e U V.
-intros e x U V H1; apply sub_extensionality; trivial;
-intro X; apply sym_eq; apply get_bound_remove_var.
+    wf_env e -> sub (remove_var e x) U V -> sub e U V.
+  intros e x U V H1; apply sub_extensionality; trivial;
+    intro X; apply sym_eq; apply get_bound_remove_var.
 Qed.
 
 Lemma sub_weakening_var :
   forall (e : env) (T U V : typ),
-  wf_typ e V -> sub e T U -> sub (evar e V) T U.
-intros e T U V H1 H2; generalize H2; apply sub_extensionality; trivial;
-simpl; split; trivial; exact (proj1 (sub_wf H2)).
+    wf_typ e V -> sub e T U -> sub (evar e V) T U.
+  intros e T U V H1 H2; generalize H2; apply sub_extensionality; trivial;
+    simpl; split; trivial; exact (proj1 (sub_wf H2)).
 Qed.
 
 (****)
@@ -852,74 +982,74 @@ Qed.
 (*
    The environments E,X <: Q,E' and E,X<:P,E' are in a narrowing relation
    if E |- P <: Q.
-*)
+ *)
 
 Inductive narrow : nat -> env -> env -> Prop :=
-    narrow_0 :
-      forall (e : env) (T T' : typ),
+  narrow_0 :
+    forall (e : env) (T T' : typ),
       sub e T' T -> narrow 0 (ebound e T) (ebound e T')
-  | narrow_extend_bound :
-      forall (e e' : env) (T : typ) (X : nat),
-      wf_typ e' T -> narrow X e e' ->
-      narrow (1 + X) (ebound e T) (ebound e' T)
-  | narrow_extend_var :
-      forall (e e' : env) (T : typ) (X : nat),
-      wf_typ e' T -> narrow X e e' -> narrow X (evar e T) (evar e' T).
+| narrow_extend_bound :
+  forall (e e' : env) (T : typ) (X : nat),
+    wf_typ e' T -> narrow X e e' ->
+    narrow (1 + X) (ebound e T) (ebound e' T)
+| narrow_extend_var :
+  forall (e e' : env) (T : typ) (X : nat),
+    wf_typ e' T -> narrow X e e' -> narrow X (evar e T) (evar e' T).
 
 Lemma get_bound_narrow_ne :
   forall (X X' : nat) (e e' : env),
-  narrow X e e' -> X' <> X -> get_bound e X' = get_bound e' X'.
-intros n n' e e' H; generalize n'; clear n'; induction H; intros n' H1; simpl;
-  [ induction n'; trivial; case H1; trivial
-  | induction n'; trivial; rewrite IHnarrow; trivial; lia
-  | auto ].
+    narrow X e e' -> X' <> X -> get_bound e X' = get_bound e' X'.
+  intros n n' e e' H; generalize n'; clear n'; induction H; intros n' H1; simpl;
+    [ induction n'; trivial; case H1; trivial
+    | induction n'; trivial; rewrite IHnarrow; trivial; lia
+    | auto ].
 Qed.
 
 Lemma get_bound_narrow_eq :
   forall (X : nat) (e e' : env),
-  narrow X e e' ->
-  exists T, exists T',
-  get_bound e X = Some T /\ get_bound e' X = Some T' /\ sub e' T' T.
-intros n e e' H; induction H;
-  [ exists (tshift 0 T); exists (tshift 0 T'); repeat split;
-    apply sub_weakening_bound; trivial; exact (proj1 (proj2 (sub_wf H)))
-  | generalize IHnarrow; intros (Q, (P, (H1, (H2, H3))));
-    exists (tshift 0 Q); exists (tshift 0 P); simpl; repeat split;
-      [ rewrite H1; trivial
-      | rewrite H2; trivial
-      | apply sub_weakening_bound; trivial ]
-  | generalize IHnarrow; intros (Q, (P, (H1, (H2, H3))));
-    exists Q; exists P; repeat split; trivial;
-    apply sub_weakening_var; trivial ].
+    narrow X e e' ->
+    exists T, exists T',
+      get_bound e X = Some T /\ get_bound e' X = Some T' /\ sub e' T' T.
+  intros n e e' H; induction H;
+    [ exists (tshift 0 T); exists (tshift 0 T'); repeat split;
+             apply sub_weakening_bound; trivial; exact (proj1 (proj2 (sub_wf H)))
+      | generalize IHnarrow; intros (Q, (P, (H1, (H2, H3))));
+        exists (tshift 0 Q); exists (tshift 0 P); simpl; repeat split;
+        [ rewrite H1; trivial
+        | rewrite H2; trivial
+        | apply sub_weakening_bound; trivial ]
+      | generalize IHnarrow; intros (Q, (P, (H1, (H2, H3))));
+        exists Q; exists P; repeat split; trivial;
+        apply sub_weakening_var; trivial ].
 Qed.
 
 Lemma get_var_narrow :
   forall (X x' : nat) (e e' : env),
-  narrow X e e' -> get_var e x' = get_var e' x'.
-intros n n' e e' H; generalize n'; clear n'; induction H;
-  [ trivial
-  | simpl; intros n'; rewrite IHnarrow; trivial
-  | simpl; induction n'; trivial ].
+    narrow X e e' -> get_var e x' = get_var e' x'.
+  intros n n' e e' H; generalize n'; clear n'; induction H;
+    [ trivial
+    | simpl; intros n'; rewrite IHnarrow; trivial
+    | simpl; induction n'; trivial ].
 Qed.
 
 Lemma narrow_wf_typ :
   forall (e e' : env) (T : typ) (X : nat),
-  narrow X e e' -> wf_typ e T -> wf_typ e' T.
-intros e e' T n H1 H2;
-apply wf_typ_env_weaken with (2 := H2); intros n' H3;
-case (eq_nat_dec n' n);
-  [ intros E; rewrite E in H3;
-    generalize (get_bound_narrow_eq H1);
-    intros (Q, (P, (H4, (H5, H6)))); rewrite H5 in H3; discriminate
-  | intro H4; rewrite (get_bound_narrow_ne H1 H4); trivial ].
+    narrow X e e' -> wf_typ e T -> wf_typ e' T.
+  intros e e' T n H1 H2;
+    apply wf_typ_env_weaken with (2 := H2); intros n' H3;
+    case (eq_nat_dec n' n);
+    [ intros E; rewrite E in H3;
+      generalize (get_bound_narrow_eq H1);
+      intros (Q, (P, (H4, (H5, H6)))); rewrite H5 in H3; discriminate
+    | intro H4; rewrite (get_bound_narrow_ne H1 H4); trivial ].
 Qed.
 
 Lemma narrow_wf_env :
   forall (e e' : env) (X : nat),
-  narrow X e e' -> wf_env e -> wf_env e'.
-intros e e' n H; induction H; simpl;
-intros (H1, H2); split; auto;
-exact (proj1 (proj2 (sub_wf H))).
+    narrow X e e' -> wf_env e -> wf_env e'.
+  intros e e' n H; induction H; simpl;
+    intros (H1, H2); split; auto;
+    exact (proj1 (proj2 (sub_wf H))).
 Qed.
 
 (****)
@@ -934,8 +1064,8 @@ Definition transitivity_prop (Q : typ) :=
 
 Definition narrowing_prop (Q : typ) :=
   forall (e e' : env) (X : nat) (S T : typ),
-  narrow X e e' -> get_bound e X = Some Q ->
-  sub e S T -> sub e' S T.
+    narrow X e e' -> get_bound e X = Some Q ->
+    sub e S T -> sub e' S T.
 
 (* The proof follows closely the paper proof.  However, we cannot
    perform a proof on the distinguished type [Q] as the induction in
@@ -951,9 +1081,9 @@ Fixpoint size (T : typ) : nat :=
   end.
 
 Lemma shift_preserves_size :
- forall (T : typ) (X : nat), size (tshift X T) = size T.
-induction T; trivial;
-simpl; intros n; rewrite IHT1; rewrite IHT2; trivial.
+  forall (T : typ) (X : nat), size (tshift X T) = size T.
+  induction T; trivial;
+    simpl; intros n; rewrite IHT1; rewrite IHT2; trivial.
 Qed.
 
 (* Now we give the crucial step in the proof of transitivity, showing
@@ -962,45 +1092,45 @@ Qed.
 
 Lemma transitivity_case :
   forall Q : typ,
-  (forall Q' : typ,
-   size Q' < size Q -> transitivity_prop Q' /\ narrowing_prop Q') ->
-  transitivity_prop Q.
-intros Q H e S T H1 H2; induction H1;
-  [ inversion_clear H2; apply SA_Top; trivial
-  | trivial
-  | exact (SA_Trans_TVar H0 (IHsub H H2))
-  | inversion_clear H2;
+    (forall Q' : typ,
+        size Q' < size Q -> transitivity_prop Q' /\ narrowing_prop Q') ->
+    transitivity_prop Q.
+  intros Q H e S T H1 H2; induction H1;
+    [ inversion_clear H2; apply SA_Top; trivial
+    | trivial
+    | exact (SA_Trans_TVar H0 (IHsub H H2))
+    | inversion_clear H2;
       [ apply SA_Top; trivial;
         simpl; split;
-          [ apply (proj2 (proj2 (sub_wf H1_)))
-          | apply (proj1 (proj2 (sub_wf H1_0))) ]
+        [ apply (proj2 (proj2 (sub_wf H1_)))
+        | apply (proj1 (proj2 (sub_wf H1_0))) ]
       | apply SA_Arrow;
-          [ assert (H5 : size T1 < size (arrow T1 T2)); try (simpl; lia);
-            generalize (H _ H5); intros (H6, _); exact (H6 _ _ _ H0 H1_)
-          | assert (H5 : size T2 < size (arrow T1 T2)); try (simpl; lia);
-            generalize (H _ H5); intros (H6, _);
-            exact (H6 _ _ _ H1_0 H1) ] ]
-  | inversion_clear H2;
+        [ assert (H5 : size T1 < size (arrow T1 T2)); try (simpl; lia);
+          generalize (H _ H5); intros (H6, _); exact (H6 _ _ _ H0 H1_)
+        | assert (H5 : size T2 < size (arrow T1 T2)); try (simpl; lia);
+          generalize (H _ H5); intros (H6, _);
+          exact (H6 _ _ _ H1_0 H1) ] ]
+    | inversion_clear H2;
       [ apply SA_Top; trivial;
         simpl; split;
-          [ apply (proj2 (proj2 (sub_wf H1_)))
-          | apply wf_typ_ebound with (U := T1);
-            apply (proj1 (proj2 (sub_wf H1_0))) ]
+        [ apply (proj2 (proj2 (sub_wf H1_)))
+        | apply wf_typ_ebound with (U := T1);
+          apply (proj1 (proj2 (sub_wf H1_0))) ]
       | assert (H5 : size T1 < size (all T1 T2)); try (simpl; lia);
         apply SA_All;
-          [ generalize (H _ H5); intros (H6, _); exact (H6 _ _ _ H0 H1_)
-          | assert (H5' : size (tshift 0 T1) < size (all T1 T2));
-              [ rewrite shift_preserves_size; trivial
-              | generalize (H _ H5'); intros (_, H6);
-                assert (H7 := narrow_0 H0);
-                assert
-                  (H7' : get_bound (ebound e T1) 0 = Some (tshift 0 T1));
-                  [ trivial
-                  | assert (H8 := H6 _ _ _ _ _ H7 H7' H1_0);
-                    assert (H9 : size T2 < size (all T1 T2));
-                    try (simpl; lia);
-                    assert (G1 := proj1 (H _ H9));
-                    exact (G1 (ebound e T0) _ _ H8 H1) ] ] ] ] ].
+        [ generalize (H _ H5); intros (H6, _); exact (H6 _ _ _ H0 H1_)
+        | assert (H5' : size (tshift 0 T1) < size (all T1 T2));
+          [ rewrite shift_preserves_size; trivial
+          | generalize (H _ H5'); intros (_, H6);
+            assert (H7 := narrow_0 H0);
+            assert
+              (H7' : get_bound (ebound e T1) 0 = Some (tshift 0 T1));
+            [ trivial
+            | assert (H8 := H6 _ _ _ _ _ H7 H7' H1_0);
+              assert (H9 : size T2 < size (all T1 T2));
+              try (simpl; lia);
+              assert (G1 := proj1 (H _ H9));
+              exact (G1 (ebound e T0) _ _ H8 H1) ] ] ] ] ].
 Qed.
 
 (* Next we give the crucial step in the proof of narrowing, showing
@@ -1010,17 +1140,17 @@ Qed.
 
 Lemma narrowing_case :
   forall Q : typ,
-  (forall Q' : typ, size Q' = size Q -> transitivity_prop Q') ->
-  narrowing_prop Q.
-intros Q H2 e e' n T1 T2 H3 H4 H5; generalize e' n H3 H4; clear e' n H3 H4;
-generalize Q H2; clear Q H2; induction H5; intros Q H2 e' n H3 H4;
-  [ apply SA_Top;
+    (forall Q' : typ, size Q' = size Q -> transitivity_prop Q') ->
+    narrowing_prop Q.
+  intros Q H2 e e' n T1 T2 H3 H4 H5; generalize e' n H3 H4; clear e' n H3 H4;
+    generalize Q H2; clear Q H2; induction H5; intros Q H2 e' n H3 H4;
+    [ apply SA_Top;
       [ exact (narrow_wf_env H3 H)
       | exact (narrow_wf_typ H3 H0) ]
-  | apply SA_Refl_TVar;
+    | apply SA_Refl_TVar;
       [ exact (narrow_wf_env H3 H)
       | exact (narrow_wf_typ H3 H0) ]
-  | case (eq_nat_dec X n);
+    | case (eq_nat_dec X n);
       [ intro E; rewrite E in H; rewrite E; clear X E;
         assert (H4' := IHsub _ H2 _ _ H3 H4);
         rewrite H in H4; injection H4; intro E; rewrite E in H4';
@@ -1033,15 +1163,15 @@ generalize Q H2; clear Q H2; induction H5; intros Q H2 e' n H3 H4;
         apply SA_Trans_TVar with (2 := H8); trivial
       | intro H6; apply SA_Trans_TVar with (2 := IHsub _ H2 _ _ H3 H4);
         rewrite <- (get_bound_narrow_ne H3 H6); trivial ]
- | apply SA_Arrow; eauto
- | apply SA_All;
-     [ eauto
-     | apply IHsub2 with (Q := tshift 0 Q) (n := (1 + n));
-         [ intros Q' E; apply H2; rewrite E; apply shift_preserves_size
-         | apply narrow_extend_bound with (2 := H3);
-           apply narrow_wf_typ with (1 := H3);
-           exact (proj1 (proj2 (sub_wf H5_)))
-         | simpl; rewrite H4; trivial ] ] ].
+    | apply SA_Arrow; eauto
+    | apply SA_All;
+      [ eauto
+      | apply IHsub2 with (Q := tshift 0 Q) (n := (1 + n));
+        [ intros Q' E; apply H2; rewrite E; apply shift_preserves_size
+        | apply narrow_extend_bound with (2 := H3);
+          apply narrow_wf_typ with (1 := H3);
+          exact (proj1 (proj2 (sub_wf H5_)))
+        | simpl; rewrite H4; trivial ] ] ].
 Qed.
 
 (* Now we combine the above lemmas into the full proof of transitivity
@@ -1050,35 +1180,35 @@ Qed.
    induction on q.) *)
 
 Lemma transitivity_and_narrowing :
- forall Q : typ, transitivity_prop Q /\ narrowing_prop Q.
-assert
- (H :
-  forall (n : nat) (Q : typ),
-  size Q < n -> transitivity_prop Q /\ narrowing_prop Q);
- [ induction n;
-    [ intros Q H; assert False; [ lia | contradiction ]
-    | intros Q H; case (le_lt_or_eq _ _ H);
-       [ intro H'; apply IHn; lia
-       | intro E; injection E; clear E; intro E; rewrite <- E in IHn;
+  forall Q : typ, transitivity_prop Q /\ narrowing_prop Q.
+  assert
+    (H :
+      forall (n : nat) (Q : typ),
+        size Q < n -> transitivity_prop Q /\ narrowing_prop Q);
+    [ induction n;
+      [ intros Q H; assert False; [ lia | contradiction ]
+      | intros Q H; case (le_lt_or_eq _ _ H);
+        [ intro H'; apply IHn; lia
+        | intro E; injection E; clear E; intro E; rewrite <- E in IHn;
           assert
-           (H1 : forall Q' : typ, size Q' = size Q -> transitivity_prop Q');
+            (H1 : forall Q' : typ, size Q' = size Q -> transitivity_prop Q');
           [ intros Q' E1; rewrite <- E1 in IHn; apply transitivity_case;
-             trivial
+            trivial
           | split; [ apply H1; trivial | apply narrowing_case; trivial ] ] ] ]
- | intro Q; apply (H (S (size Q))); lia ].
+    | intro Q; apply (H (S (size Q))); lia ].
 Qed.
 
 Lemma sub_transitivity :
   forall (e : env) (T U V : typ), sub e T U -> sub e U V -> sub e T V.
-intros e T U; apply (proj1 (transitivity_and_narrowing U)).
+  intros e T U; apply (proj1 (transitivity_and_narrowing U)).
 Qed.
 
 Lemma sub_narrowing :
   forall (e e' : env) (X : nat) (S T : typ),
-  narrow X e e' -> sub e S T -> sub e' S T.
-intros e e' n S T H1 H2;
-generalize (get_bound_narrow_eq H1); intros (Q, (P, (H3, _)));
-exact (proj2 (transitivity_and_narrowing Q) _ _ _ _ _ H1 H3 H2).
+    narrow X e e' -> sub e S T -> sub e' S T.
+  intros e e' n S T H1 H2;
+    generalize (get_bound_narrow_eq H1); intros (Q, (P, (H3, _)));
+    exact (proj2 (transitivity_and_narrowing Q) _ _ _ _ _ H1 H3 H2).
 Qed.
 
 
@@ -1094,64 +1224,64 @@ Qed.
       E, X <: T, E'  |-->  E, [X|->T']E',
    assuming that E |- T' <: T.
    (see definition A.9)
-*)
+ *)
 
 Inductive env_subst : nat -> typ -> env -> env -> Prop :=
-    es_here :
-      forall (e : env) (T T' : typ),
+  es_here :
+    forall (e : env) (T T' : typ),
       sub e T' T -> env_subst 0 T' (ebound e T) e
-  | es_var :
-      forall (X : nat) (T T' : typ) (e e' : env),
-      env_subst X T' e e' ->
-      env_subst X T' (evar e T) (evar e' (tsubst T X T'))
-  | es_bound :
-      forall (X : nat) (T T' : typ) (e e' : env),
-      env_subst X T' e e' ->
-      env_subst (1 + X) (tshift 0 T') (ebound e T) (ebound e' (tsubst T X T')).
+| es_var :
+  forall (X : nat) (T T' : typ) (e e' : env),
+    env_subst X T' e e' ->
+    env_subst X T' (evar e T) (evar e' (tsubst T X T'))
+| es_bound :
+  forall (X : nat) (T T' : typ) (e e' : env),
+    env_subst X T' e e' ->
+    env_subst (1 + X) (tshift 0 T') (ebound e T) (ebound e' (tsubst T X T')).
 
 Lemma env_subst_get_var :
   forall (x X' : nat) (e e' : env) (T : typ),
-  (env_subst  X' T e e') ->
-  get_var e' x = opt_map (fun T' => tsubst T' X' T) (get_var e x).
-intros n n' e e' T H; generalize n; clear n; induction H;
-  [ intro n; simpl; induction (get_var e n); simpl; trivial;
-    apply f_equal with (f := @Some typ); apply tsubst_tshift_prop
-  | intro n'; induction n'; simpl; trivial
-  | simpl; intro n'; rewrite IHenv_subst;
-    induction (get_var e n'); simpl; trivial;
-    apply f_equal with (f := @Some typ);
-    apply (tshift_tsubst_prop_1 0 X) ].
+    (env_subst  X' T e e') ->
+    get_var e' x = opt_map (fun T' => tsubst T' X' T) (get_var e x).
+  intros n n' e e' T H; generalize n; clear n; induction H;
+    [ intro n; simpl; induction (get_var e n); simpl; trivial;
+      apply f_equal with (f := @Some typ); apply tsubst_tshift_prop
+    | intro n'; induction n'; simpl; trivial
+    | simpl; intro n'; rewrite IHenv_subst;
+      induction (get_var e n'); simpl; trivial;
+      apply f_equal with (f := @Some typ);
+      apply (tshift_tsubst_prop_1 0 X) ].
 Qed.
 
 Lemma env_subst_get_bound_lt :
   forall (X X' : nat) (e e' : env) (T : typ),
-  (env_subst X' T e e') -> X < X' ->
-  get_bound e' X = opt_map (fun T' => tsubst T' X' T) (get_bound e X).
-intros n n' e e' T H; generalize n; clear n;
-induction H; simpl; trivial; intros n' H1;
-  [ inversion H1
-  | induction n';
+    (env_subst X' T e e') -> X < X' ->
+    get_bound e' X = opt_map (fun T' => tsubst T' X' T) (get_bound e X).
+  intros n n' e e' T H; generalize n; clear n;
+    induction H; simpl; trivial; intros n' H1;
+    [ inversion H1
+    | induction n';
       [ simpl; apply f_equal with (f := @Some typ);
         apply (tshift_tsubst_prop_1 0 X)
       | clear IHn'; rewrite IHenv_subst;
-          [ case (get_bound e n'); simpl; trivial; intro T'';
-            apply f_equal with (f := @Some typ);
-            apply (tshift_tsubst_prop_1 0 X)
-          | lia ] ] ].
+        [ case (get_bound e n'); simpl; trivial; intro T'';
+          apply f_equal with (f := @Some typ);
+          apply (tshift_tsubst_prop_1 0 X)
+        | lia ] ] ].
 Qed.
 
 Lemma env_subst_get_bound_ge :
   forall (X X' : nat) (e e' : env) (T : typ),
-  env_subst X' T e e' -> X' < X ->
-  get_bound e' (X - 1) = opt_map (fun T' => tsubst T' X' T) (get_bound e X).
-intros n n' e e' T H; generalize n; clear n;
-induction H; simpl; trivial; intros n' H1;
-  [ induction n';
+    env_subst X' T e e' -> X' < X ->
+    get_bound e' (X - 1) = opt_map (fun T' => tsubst T' X' T) (get_bound e X).
+  intros n n' e e' T H; generalize n; clear n;
+    induction H; simpl; trivial; intros n' H1;
+    [ induction n';
       [ inversion H1
       | simpl; rewrite <- minus_n_O; case (get_bound e n'); simpl; trivial;
         intro T''; apply f_equal with (f := @Some typ);
         apply tsubst_tshift_prop ]
-  | induction n';
+    | induction n';
       [ inversion H1
       | clear IHn'; replace ((S n') - 1) with (S (n' - 1)); try lia;
         rewrite IHenv_subst; try lia;
@@ -1162,39 +1292,39 @@ Qed.
 
 Lemma env_subst_wf_typ_0 :
   forall (e e' : env) (T : typ) (X : nat),
-  env_subst X T e e' -> wf_env e' -> wf_typ e' T.
-intros e e' T X H; induction H; simpl;
-  [ intros _; exact (proj1 (proj2 (sub_wf H)))
-  | intros (H1, H2); apply wf_typ_weakening_var; auto
-  | intros (H1, H2); apply wf_typ_weakening_bound; auto ].
+    env_subst X T e e' -> wf_env e' -> wf_typ e' T.
+  intros e e' T X H; induction H; simpl;
+    [ intros _; exact (proj1 (proj2 (sub_wf H)))
+    | intros (H1, H2); apply wf_typ_weakening_var; auto
+    | intros (H1, H2); apply wf_typ_weakening_bound; auto ].
 Qed.
 
 Lemma env_subst_wf_typ :
   forall (e e' : env) (S T : typ) (X : nat),
-  env_subst X T e e' -> wf_typ e S -> wf_env e' -> wf_typ e' (tsubst S X T).
-intros e e' S; generalize e e'; clear e e'; induction S;
-  [ intros e e' T n' H1 H2 H3; simpl; simpl in H2; case (lt_eq_lt_dec n n');
+    env_subst X T e e' -> wf_typ e S -> wf_env e' -> wf_typ e' (tsubst S X T).
+  intros e e' S; generalize e e'; clear e e'; induction S;
+    [ intros e e' T n' H1 H2 H3; simpl; simpl in H2; case (lt_eq_lt_dec n n');
       [ intro s; case s; clear s; intro H5;
-          [ simpl; rewrite env_subst_get_bound_lt with (1 := H1) (2 := H5);
-            induction (get_bound e n); trivial; discriminate
-          | exact (env_subst_wf_typ_0 H1 H3) ]
+        [ simpl; rewrite env_subst_get_bound_lt with (1 := H1) (2 := H5);
+          induction (get_bound e n); trivial; discriminate
+        | exact (env_subst_wf_typ_0 H1 H3) ]
       | intro H5; simpl;
         rewrite env_subst_get_bound_ge with (1 := H1) (2 := H5);
         induction (get_bound e n); trivial; discriminate ]
-  | trivial
-  | simpl; intros e e' T n H0 (H1, H2) H3; eauto
-  | simpl; intros e e' T n H0 (H1, H2) H3; split; eauto;
-    apply IHS2 with (e := (ebound e S1)); trivial;
+    | trivial
+    | simpl; intros e e' T n H0 (H1, H2) H3; eauto
+    | simpl; intros e e' T n H0 (H1, H2) H3; split; eauto;
+      apply IHS2 with (e := (ebound e S1)); trivial;
       [ exact (es_bound S1 H0)
       | simpl; split; trivial; apply IHS1 with (1 := H0); trivial ] ].
 Qed.
 
 Lemma env_subst_wf_env :
   forall (e e' : env) (T : typ) (X : nat),
-  env_subst X T e e' -> wf_env e -> wf_env e'.
-intros e e' T X H; induction H; simpl; try tauto;
-intros (H1, H2); split; auto;
-apply env_subst_wf_typ with (1 := H); auto.
+    env_subst X T e e' -> wf_env e -> wf_env e'.
+  intros e e' T X H; induction H; simpl; try tauto;
+    intros (H1, H2); split; auto;
+    apply env_subst_wf_typ with (1 := H); auto.
 Qed.
 
 (****)
@@ -1203,19 +1333,19 @@ Qed.
 
 Lemma typing_wf :
   forall (e : env) (t : term) (U : typ),
-  typing e t U -> wf_env e /\ wf_term e t /\ wf_typ e U.
-intros e t U H; induction H;
-  [ repeat split; simpl; trivial;
+    typing e t U -> wf_env e /\ wf_term e t /\ wf_typ e U.
+  intros e t U H; induction H;
+    [ repeat split; simpl; trivial;
       [ simpl; rewrite H0; discriminate
       | exact (get_var_wf H H0) ]
-  | simpl in IHtyping; simpl; repeat split; try tauto;
-    apply wf_typ_strengthening_var with (T := T1); tauto
-  | simpl; simpl in IHtyping1; tauto
-  | simpl; simpl in IHtyping; tauto
-  | simpl; simpl in IHtyping; assert (H1 := proj1 (proj2 (sub_wf H0)));
-    repeat split; try tauto;
-    apply env_subst_wf_typ with (1 := es_here H0); tauto
-  | repeat split; try tauto; exact (proj2 (proj2 (sub_wf H0))) ].
+    | simpl in IHtyping; simpl; repeat split; try tauto;
+      apply wf_typ_strengthening_var with (T := T1); tauto
+    | simpl; simpl in IHtyping1; tauto
+    | simpl; simpl in IHtyping; tauto
+    | simpl; simpl in IHtyping; assert (H1 := proj1 (proj2 (sub_wf H0)));
+      repeat split; try tauto;
+      apply env_subst_wf_typ with (1 := es_here H0); tauto
+    | repeat split; try tauto; exact (proj2 (proj2 (sub_wf H0))) ].
 Qed.
 
 (****)
@@ -1230,63 +1360,63 @@ Qed.
 
 Lemma typing_weakening_bound_ind :
   forall (e e' : env) (X : nat) (t : term) (U : typ),
-  insert_bound X e e' ->
-  typing e t U -> typing e' (shift_typ X t) (tshift X U).
-intros e e' n t U H1 H2; generalize n e' H1; clear n e' H1;
-induction H2; intros n1 e' H1; simpl;
-  [ apply T_Var;
+    insert_bound X e e' ->
+    typing e t U -> typing e' (shift_typ X t) (tshift X U).
+  intros e e' n t U H1 H2; generalize n e' H1; clear n e' H1;
+    induction H2; intros n1 e' H1; simpl;
+    [ apply T_Var;
       [ exact (insert_bound_wf_env H1 H)
       | rewrite get_var_insert_bound with (1 := H1); rewrite H0; trivial ]
-  | apply T_Abs; apply IHtyping; apply ib_var; trivial
-  | assert (H2 := (IHtyping1 _ _ H1)); assert (H3 := (IHtyping2 _ _ H1));
-    exact (T_App H2 H3)
-  | apply T_Tabs; apply IHtyping; exact (ib_bound T1 H1)
-  | rewrite (tshift_tsubst_prop_2 0 n1);
-    apply (T_Tapp (IHtyping _ _ H1) (sub_weakening_bound_ind H1 H))
-  | exact (T_Sub (IHtyping _ _ H1) (sub_weakening_bound_ind H1 H)) ].
+    | apply T_Abs; apply IHtyping; apply ib_var; trivial
+    | assert (H2 := (IHtyping1 _ _ H1)); assert (H3 := (IHtyping2 _ _ H1));
+      exact (T_App H2 H3)
+    | apply T_Tabs; apply IHtyping; exact (ib_bound T1 H1)
+    | rewrite (tshift_tsubst_prop_2 0 n1);
+      apply (T_Tapp (IHtyping _ _ H1) (sub_weakening_bound_ind H1 H))
+    | exact (T_Sub (IHtyping _ _ H1) (sub_weakening_bound_ind H1 H)) ].
 Qed.
 
 Lemma typing_weakening_bound :
   forall (e : env) (t : term) (U V : typ),
-  wf_typ e V -> typing e t U ->
-  typing (ebound e V) (shift_typ 0 t) (tshift 0 U).
-intros e t U V H1 H2; apply typing_weakening_bound_ind with (2 := H2);
-apply ib_here; trivial.
+    wf_typ e V -> typing e t U ->
+    typing (ebound e V) (shift_typ 0 t) (tshift 0 U).
+  intros e t U V H1 H2; apply typing_weakening_bound_ind with (2 := H2);
+    apply ib_here; trivial.
 Qed.
 
 Lemma typing_weakening_var_ind :
   forall (e : env) (x : nat) (t : term) (U : typ),
-  wf_env e -> typing (remove_var e x) t U -> typing e (shift x t) U.
-intros e n t U H1 H2; cut (exists e', e' = remove_var e n);
-  [ intros (e', E); rewrite <- E in H2; generalize n e E H1; clear n e E H1;
-    induction H2; intros n' e' E H1; simpl;
+    wf_env e -> typing (remove_var e x) t U -> typing e (shift x t) U.
+  intros e n t U H1 H2; cut (exists e', e' = remove_var e n);
+    [ intros (e', E); rewrite <- E in H2; generalize n e E H1; clear n e E H1;
+      induction H2; intros n' e' E H1; simpl;
       [ apply T_Var; trivial; rewrite E in H0;
         case (le_gt_dec n' x); intro H2;
-          [ rewrite get_var_remove_var_ge in H0; trivial; lia
-          | rewrite get_var_remove_var_lt in H0; trivial; lia ]
+        [ rewrite get_var_remove_var_ge in H0; trivial; lia
+        | rewrite get_var_remove_var_lt in H0; trivial; lia ]
       | apply T_Abs; apply IHtyping;
-          [ rewrite E; trivial
-          | simpl; split; trivial;
-            assert (H3 := proj1 (proj1 (typing_wf H2))); rewrite E in H3;
-            exact (wf_typ_insert_var H3) ]
+        [ rewrite E; trivial
+        | simpl; split; trivial;
+          assert (H3 := proj1 (proj1 (typing_wf H2))); rewrite E in H3;
+          exact (wf_typ_insert_var H3) ]
       | exact (T_App (IHtyping1 _ _ E H1) (IHtyping2 _ _ E H1))
       | apply T_Tabs; apply IHtyping;
-          [ rewrite E; trivial
-          | simpl; split; trivial;
-            assert (H3 := proj1 (proj1 (typing_wf H2))); rewrite E in H3;
-            exact (wf_typ_insert_var H3) ]
+        [ rewrite E; trivial
+        | simpl; split; trivial;
+          assert (H3 := proj1 (proj1 (typing_wf H2))); rewrite E in H3;
+          exact (wf_typ_insert_var H3) ]
       | apply (T_Tapp (T2 := T2) (IHtyping _ _ E H1));
         rewrite E in H; exact (sub_weakening_var_ind H1 H)
       | apply (T_Sub (T2 := T2) (IHtyping _ _ E H1));
         rewrite E in H; exact (sub_weakening_var_ind H1 H) ]
-  | exists (remove_var e n); trivial ].
+    | exists (remove_var e n); trivial ].
 Qed.
 
 Lemma typing_weakening_var :
   forall (e : env) (t : term) (U V : typ),
-  wf_typ e V -> typing e t U -> typing (evar e V) (shift 0 t) U.
-intros e t U V H1 H2; apply (@typing_weakening_var_ind (evar e V));
-simpl; trivial; split; trivial; exact (proj1 (typing_wf H2)).
+    wf_typ e V -> typing e t U -> typing (evar e V) (shift 0 t) U.
+  intros e t U V H1 H2; apply (@typing_weakening_var_ind (evar e V));
+    simpl; trivial; split; trivial; exact (proj1 (typing_wf H2)).
 Qed.
 
 (****)
@@ -1295,10 +1425,10 @@ Qed.
 
 Lemma sub_strengthening_var :
   forall (e : env) (x : nat) (U V : typ),
-  sub e U V -> sub (remove_var e x) U V.
-intros e x U V H1; generalize H1; apply sub_extensionality;
-  [ intro X; apply get_bound_remove_var
-  | apply wf_env_remove_var; exact (proj1 (sub_wf H1)) ].
+    sub e U V -> sub (remove_var e x) U V.
+  intros e x U V H1; generalize H1; apply sub_extensionality;
+    [ intro X; apply get_bound_remove_var
+    | apply wf_env_remove_var; exact (proj1 (sub_wf H1)) ].
 Qed.
 
 (****)
@@ -1307,27 +1437,27 @@ Qed.
 
 Lemma typing_narrowing_ind :
   forall (e e' : env) (X : nat) (t : term) (U : typ),
-  narrow X e e' -> typing e t U -> typing e' t U.
-intros e e' n t U H1 H2; generalize e' n H1; clear e' n H1;
-induction H2; intros e' n1 H1;
-  [ apply T_Var;
+    narrow X e e' -> typing e t U -> typing e' t U.
+  intros e e' n t U H1 H2; generalize e' n H1; clear e' n H1;
+    induction H2; intros e' n1 H1;
+    [ apply T_Var;
       [ exact (narrow_wf_env H1 H)
       | rewrite <- get_var_narrow with (1 := H1); trivial ]
-  | apply T_Abs; apply IHtyping with (n := n1);
-    apply narrow_extend_var; trivial;
-    exact (narrow_wf_typ H1 (proj1 (proj1 (typing_wf H2))))
-  | eapply T_App; eauto
-  | apply T_Tabs; apply IHtyping with (n := S n1);
-    apply narrow_extend_bound with (X := n1); trivial;
-    exact (narrow_wf_typ H1 (proj1 (proj1 (typing_wf H2))))
-  | eapply T_Tapp; eauto; exact (sub_narrowing H1 H)
-  | apply T_Sub with (1 := IHtyping _ _ H1); exact (sub_narrowing H1 H) ].
+    | apply T_Abs; apply IHtyping with (n := n1);
+      apply narrow_extend_var; trivial;
+      exact (narrow_wf_typ H1 (proj1 (proj1 (typing_wf H2))))
+    | eapply T_App; eauto
+    | apply T_Tabs; apply IHtyping with (n := S n1);
+      apply narrow_extend_bound with (X := n1); trivial;
+      exact (narrow_wf_typ H1 (proj1 (proj1 (typing_wf H2))))
+    | eapply T_Tapp; eauto; exact (sub_narrowing H1 H)
+    | apply T_Sub with (1 := IHtyping _ _ H1); exact (sub_narrowing H1 H) ].
 Qed.
 
 Lemma typing_narrowing :
- forall (e : env) (t : term) (U V1 V2 : typ),
- typing (ebound e V1) t U -> sub e V2 V1 -> typing (ebound e V2) t U.
-intros e t U V1 V2 H1 H2; exact (typing_narrowing_ind (narrow_0 H2) H1).
+  forall (e : env) (t : term) (U V1 V2 : typ),
+    typing (ebound e V1) t U -> sub e V2 V1 -> typing (ebound e V2) t U.
+  intros e t U V1 V2 H1 H2; exact (typing_narrowing_ind (narrow_0 H2) H1).
 Qed.
 
 (****)
@@ -1341,36 +1471,36 @@ Qed.
 
 Lemma subst_preserves_typing :
   forall (e : env) (x : nat) (t u : term) (V W : typ),
-  typing e t V ->
-  typing (remove_var e x) u W -> get_var e x = Some W ->
-  typing (remove_var e x) (subst t x u) V.
-intros e n t u V W H; generalize n u W; clear n u W;
-induction H; intros n' u W H1 E1;
-  [ simpl; case (lt_eq_lt_dec x n');
+    typing e t V ->
+    typing (remove_var e x) u W -> get_var e x = Some W ->
+    typing (remove_var e x) (subst t x u) V.
+  intros e n t u V W H; generalize n u W; clear n u W;
+    induction H; intros n' u W H1 E1;
+    [ simpl; case (lt_eq_lt_dec x n');
       [ intro s; case s; clear s; intro H2;
-          [ apply T_Var;
-              [ apply wf_env_remove_var; trivial
-              | rewrite get_var_remove_var_lt with (1 := H2); trivial ]
-          | rewrite H2 in H0; rewrite H0 in E1; injection E1;
-            intro E3; rewrite E3; trivial ]
-      | intro H2; apply T_Var;
+        [ apply T_Var;
           [ apply wf_env_remove_var; trivial
-          | induction x;
-              [ inversion H2
-              | simpl; rewrite <- minus_n_O;
-                rewrite get_var_remove_var_ge; trivial; lia ] ] ]
-  | simpl; apply T_Abs; apply (IHtyping (S n') (shift 0 u) W); trivial;
-    assert (H2 := wf_typ_remove_var n' (proj1 (proj1 (typing_wf H))));
-    exact (typing_weakening_var H2 H1)
-  | exact (T_App (IHtyping1 _ u W H1 E1) (IHtyping2 _ u W H1 E1))
-  | simpl; apply T_Tabs; apply (IHtyping n' (shift_typ 0 u) (tshift 0 W));
+          | rewrite get_var_remove_var_lt with (1 := H2); trivial ]
+        | rewrite H2 in H0; rewrite H0 in E1; injection E1;
+          intro E3; rewrite E3; trivial ]
+      | intro H2; apply T_Var;
+        [ apply wf_env_remove_var; trivial
+        | induction x;
+          [ inversion H2
+          | simpl; rewrite <- minus_n_O;
+            rewrite get_var_remove_var_ge; trivial; lia ] ] ]
+    | simpl; apply T_Abs; apply (IHtyping (S n') (shift 0 u) W); trivial;
+      assert (H2 := wf_typ_remove_var n' (proj1 (proj1 (typing_wf H))));
+      exact (typing_weakening_var H2 H1)
+    | exact (T_App (IHtyping1 _ u W H1 E1) (IHtyping2 _ u W H1 E1))
+    | simpl; apply T_Tabs; apply (IHtyping n' (shift_typ 0 u) (tshift 0 W));
       [ assert (H2 := wf_typ_remove_var n' (proj1 (proj1 (typing_wf H))));
         exact (typing_weakening_bound H2 H1)
       | simpl; rewrite E1; trivial ]
-  | simpl; apply T_Tapp with (1 := (IHtyping _ u W H1 E1));
-    exact (sub_strengthening_var n' H0)
-  | simpl; apply T_Sub with (1 := (IHtyping _ u W H1 E1));
-    exact (sub_strengthening_var n' H0) ].
+    | simpl; apply T_Tapp with (1 := (IHtyping _ u W H1 E1));
+      exact (sub_strengthening_var n' H0)
+    | simpl; apply T_Sub with (1 := (IHtyping _ u W H1 E1));
+      exact (sub_strengthening_var n' H0) ].
 Qed.
 
 (****)
@@ -1379,47 +1509,47 @@ Qed.
 
 Lemma env_subst_sub :
   forall (e e' : env) (T T' : typ) (X : nat),
-  env_subst X T' e e' -> (get_bound e X) = (Some T) -> wf_env e' ->
-  (sub e' T' (tsubst T X T')).
-intros e e' T T' X H; generalize T; clear T; induction H; simpl;
-  [ intros T'' E H1; injection E; clear E; intro E; rewrite <- E;
-    rewrite <- tsubst_tshift_prop; trivial
-  | intros T'' E (H1, H2);
-    exact (sub_weakening_var H1 (IHenv_subst _ E H2))
-  | intros T'' E (H1, H2); induction (get_bound e X); try discriminate;
-    injection E; clear E; intro E; rewrite <- E;
-    rewrite <- (tshift_tsubst_prop_1 0 X);
-    apply sub_weakening_bound with (1 := H1); auto ].
+    env_subst X T' e e' -> (get_bound e X) = (Some T) -> wf_env e' ->
+    (sub e' T' (tsubst T X T')).
+  intros e e' T T' X H; generalize T; clear T; induction H; simpl;
+    [ intros T'' E H1; injection E; clear E; intro E; rewrite <- E;
+      rewrite <- tsubst_tshift_prop; trivial
+    | intros T'' E (H1, H2);
+      exact (sub_weakening_var H1 (IHenv_subst _ E H2))
+    | intros T'' E (H1, H2); induction (get_bound e X); try discriminate;
+      injection E; clear E; intro E; rewrite <- E;
+      rewrite <- (tshift_tsubst_prop_1 0 X);
+      apply sub_weakening_bound with (1 := H1); auto ].
 Qed.
 
 Lemma tsubst_preserves_subtyping :
   forall (e e' : env) (X : nat) (T U V : typ),
-  env_subst X T e e' -> sub e U V -> sub e' (tsubst U X T) (tsubst V X T).
-intros e e' n T U V H1 H2; generalize n e' T H1; clear n e' T H1; induction H2;
-  [ intros n e' T H1; apply SA_Top;
+    env_subst X T e e' -> sub e U V -> sub e' (tsubst U X T) (tsubst V X T).
+  intros e e' n T U V H1 H2; generalize n e' T H1; clear n e' T H1; induction H2;
+    [ intros n e' T H1; apply SA_Top;
       [ exact (env_subst_wf_env H1 H)
       | exact (env_subst_wf_typ H1 H0 (env_subst_wf_env H1 H)) ]
-  | intros n e' T H1; apply sub_reflexivity;
+    | intros n e' T H1; apply sub_reflexivity;
       [ exact (env_subst_wf_env H1 H)
       | exact (env_subst_wf_typ H1 H0 (env_subst_wf_env H1 H)) ]
-  | intros n e' T' H1; simpl; case (lt_eq_lt_dec X n);
+    | intros n e' T' H1; simpl; case (lt_eq_lt_dec X n);
       [ intros s; case s; clear s;
-          [ intro H5; apply SA_Trans_TVar with (U := tsubst U n T');
-              [ rewrite env_subst_get_bound_lt with (1 := H1) (2 := H5);
-                rewrite H; trivial
-              | apply IHsub; trivial ]
-          | intro E; apply sub_transitivity with (2 := IHsub _ _ _ H1);
-            rewrite E in H; apply (env_subst_sub H1 H);
-            exact (env_subst_wf_env H1 (proj1 (sub_wf H2))) ]
+        [ intro H5; apply SA_Trans_TVar with (U := tsubst U n T');
+          [ rewrite env_subst_get_bound_lt with (1 := H1) (2 := H5);
+            rewrite H; trivial
+          | apply IHsub; trivial ]
+        | intro E; apply sub_transitivity with (2 := IHsub _ _ _ H1);
+          rewrite E in H; apply (env_subst_sub H1 H);
+          exact (env_subst_wf_env H1 (proj1 (sub_wf H2))) ]
       | intro H5; apply SA_Trans_TVar with (U := tsubst U n T');
-          [ rewrite env_subst_get_bound_ge with (1 := H1); try lia;
-            induction X;
-              [ assert False; [ lia | contradiction ]
-              | simpl; rewrite H; trivial ]
-          | apply IHsub; trivial ] ]
-  | intros n e' T H1; simpl; apply SA_Arrow; auto
-  | intros n e' T H1; simpl; apply SA_All; auto;
-    exact (IHsub2 _ _ _ (es_bound T1 H1)) ].
+        [ rewrite env_subst_get_bound_ge with (1 := H1); try lia;
+          induction X;
+          [ assert False; [ lia | contradiction ]
+          | simpl; rewrite H; trivial ]
+        | apply IHsub; trivial ] ]
+    | intros n e' T H1; simpl; apply SA_Arrow; auto
+    | intros n e' T H1; simpl; apply SA_All; auto;
+      exact (IHsub2 _ _ _ (es_bound T1 H1)) ].
 Qed.
 
 (****)
@@ -1428,29 +1558,29 @@ Qed.
 
 Lemma subst_typ_preserves_typing_ind :
   forall (e e' : env) (t : term) (U P : typ) (X : nat),
-  env_subst X P e e' ->
-  typing e t U -> typing e' (subst_typ t X P) (tsubst U X P).
-intros e e' t U P n H1 H2; generalize n e' P H1; clear n e' P H1;
-induction H2;
-  [ intros n' e' P H1; simpl; apply T_Var;
+    env_subst X P e e' ->
+    typing e t U -> typing e' (subst_typ t X P) (tsubst U X P).
+  intros e e' t U P n H1 H2; generalize n e' P H1; clear n e' P H1;
+    induction H2;
+    [ intros n' e' P H1; simpl; apply T_Var;
       [ exact (env_subst_wf_env H1 H)
       | rewrite env_subst_get_var with (1 := H1); rewrite H0; trivial ]
-  | intros n e' P H1; simpl; apply T_Abs; exact (IHtyping _ _ _ (es_var _ H1))
-  | intros n e' P H1; exact (T_App (IHtyping1 _ _ _ H1) (IHtyping2 _ _ _ H1))
-  | intros n e' P H1; exact (T_Tabs (IHtyping _ _ _ (es_bound _ H1)))
-  | intros n e' P H1; simpl;
-    assert (H4 := T_Tapp (T2 := (tsubst T2 n P)) (IHtyping _ _ _ H1));
-    fold tsubst in H4; rewrite (tsubst_tsubst_prop 0 n);
-    apply H4; exact (tsubst_preserves_subtyping H1 H)
-  | intros n e' P H1; apply T_Sub with (1 := IHtyping _ _ _ H1);
-    exact (tsubst_preserves_subtyping H1 H) ].
+    | intros n e' P H1; simpl; apply T_Abs; exact (IHtyping _ _ _ (es_var _ H1))
+    | intros n e' P H1; exact (T_App (IHtyping1 _ _ _ H1) (IHtyping2 _ _ _ H1))
+    | intros n e' P H1; exact (T_Tabs (IHtyping _ _ _ (es_bound _ H1)))
+    | intros n e' P H1; simpl;
+      assert (H4 := T_Tapp (T2 := (tsubst T2 n P)) (IHtyping _ _ _ H1));
+      fold tsubst in H4; rewrite (tsubst_tsubst_prop 0 n);
+      apply H4; exact (tsubst_preserves_subtyping H1 H)
+    | intros n e' P H1; apply T_Sub with (1 := IHtyping _ _ _ H1);
+      exact (tsubst_preserves_subtyping H1 H) ].
 Qed.
 
 Lemma subst_typ_preserves_typing :
   forall (e : env) (t : term) (U P Q : typ),
-  typing (ebound e Q) t U -> sub e P Q ->
-  typing e (subst_typ t 0 P) (tsubst U 0 P).
-intros e t U P Q H1 H2; exact (subst_typ_preserves_typing_ind (es_here H2) H1).
+    typing (ebound e Q) t U -> sub e P Q ->
+    typing e (subst_typ t 0 P) (tsubst U 0 P).
+  intros e t U P Q H1 H2; exact (subst_typ_preserves_typing_ind (es_here H2) H1).
 Qed.
 
 (****)
@@ -1465,35 +1595,35 @@ Qed.
 
 Lemma t_abs_inversion :
   forall (e : env) (t : term) (T0 T1 T2 T3 : typ),
-  typing e (abs T1 t) T0 ->
-  sub e T0 (arrow T2 T3) ->
-  sub e T2 T1 /\
-  (exists T4, sub e T4 T3 /\ typing (evar e T1) t T4).
-intros e t T0 T1 T2 T3 H; cut (exists t' : _, t' = abs T1 t);
-  [ intros (t', E1); rewrite <- E1 in H; generalize t T1 T2 T3 E1;
-    clear t T1 T2 T3 E1;
-    induction H; intros; try discriminate;
+    typing e (abs T1 t) T0 ->
+    sub e T0 (arrow T2 T3) ->
+    sub e T2 T1 /\
+      (exists T4, sub e T4 T3 /\ typing (evar e T1) t T4).
+  intros e t T0 T1 T2 T3 H; cut (exists t' : _, t' = abs T1 t);
+    [ intros (t', E1); rewrite <- E1 in H; generalize t T1 T2 T3 E1;
+      clear t T1 T2 T3 E1;
+      induction H; intros; try discriminate;
       [ injection E1; intros E2 E3; rewrite <- E2; rewrite <- E3;
         inversion_clear H0; split; [ trivial | exists T2; split; trivial ]
       | apply IHtyping with (1 := E1) (2 := sub_transitivity H0 H1) ]
-  | exists (abs T1 t); trivial ].
+    | exists (abs T1 t); trivial ].
 Qed.
 
 Lemma t_tabs_inversion :
   forall (e : env) (t : term) (T0 T1 T2 T3 : typ),
-  typing e (tabs T1 t) T0 ->
-  sub e T0 (all T2 T3) ->
-  sub e T2 T1 /\
-  (exists T4, sub (ebound e T2) T4 T3 /\ typing (ebound e T2) t T4).
-intros e t T0 T1 T2 T3 H; cut (exists t' : _, t' = tabs T1 t);
-  [ intros (t', E1); rewrite <- E1 in H; generalize t T1 T2 T3 E1;
-    clear t T1 T2 T3 E1;
-    induction H; intros; try discriminate;
+    typing e (tabs T1 t) T0 ->
+    sub e T0 (all T2 T3) ->
+    sub e T2 T1 /\
+      (exists T4, sub (ebound e T2) T4 T3 /\ typing (ebound e T2) t T4).
+  intros e t T0 T1 T2 T3 H; cut (exists t' : _, t' = tabs T1 t);
+    [ intros (t', E1); rewrite <- E1 in H; generalize t T1 T2 T3 E1;
+      clear t T1 T2 T3 E1;
+      induction H; intros; try discriminate;
       [ injection E1; intros E2 E3; rewrite <- E2; rewrite <- E3;
         inversion_clear H0; split; trivial;
         exists T2; split; trivial; exact (typing_narrowing H H1)
       | apply IHtyping with (1 := E1) (2 := sub_transitivity H0 H1) ]
-  | exists (tabs T1 t); trivial ].
+    | exists (tabs T1 t); trivial ].
 Qed.
 
 (****)
@@ -1502,36 +1632,36 @@ Qed.
 
 Lemma fun_value :
   forall (t : term) (T1 T2 : typ),
-  value t -> typing empty t (arrow T1 T2) ->
-  exists t' , exists T1' , t = abs T1' t'.
-intros t T1 T2 H1 H; cut (exists e, e = empty);
-  [ intros (e, E1); rewrite <- E1 in H; cut (exists T0, T0 = arrow T1 T2);
+    value t -> typing empty t (arrow T1 T2) ->
+    exists t' , exists T1' , t = abs T1' t'.
+  intros t T1 T2 H1 H; cut (exists e, e = empty);
+    [ intros (e, E1); rewrite <- E1 in H; cut (exists T0, T0 = arrow T1 T2);
       [ intros (T0, E2); rewrite <- E2 in H; generalize T1 T2 E2;
         clear T1 T2 E2; induction H; try contradiction;
-          [ intros T3 T4 E; exists t; exists T1; trivial
-          | intros; discriminate
-          | intros T3 T4 E2; rewrite E2 in H0; inversion H0;
-              [ rewrite E1 in H2; induction X; discriminate
-              | exact (IHtyping H1 E1 _ _ (sym_eq H5)) ] ]
+        [ intros T3 T4 E; exists t; exists T1; trivial
+        | intros; discriminate
+        | intros T3 T4 E2; rewrite E2 in H0; inversion H0;
+          [ rewrite E1 in H2; induction X; discriminate
+          | exact (IHtyping H1 E1 _ _ (sym_eq H5)) ] ]
       | exists (arrow T1 T2); trivial ]
-  | exists empty; trivial ].
+    | exists empty; trivial ].
 Qed.
 
 Lemma typefun_value :
   forall (t : term) (T1 T2 : typ),
-  value t -> typing empty t (all T1 T2) ->
-  exists t', exists T1', t = tabs T1' t'.
-intros t T1 T2 H1 H; cut (exists e, e = empty);
-  [ intros (e, E1); rewrite <- E1 in H; cut (exists T0, T0 = all T1 T2);
+    value t -> typing empty t (all T1 T2) ->
+    exists t', exists T1', t = tabs T1' t'.
+  intros t T1 T2 H1 H; cut (exists e, e = empty);
+    [ intros (e, E1); rewrite <- E1 in H; cut (exists T0, T0 = all T1 T2);
       [ intros (T0, E2); rewrite <- E2 in H; generalize T1 T2 E2;
         clear T1 T2 E2; induction H; try contradiction;
-          [ intros; discriminate
-          | intros T3 T4 E; exists t; exists T1; trivial
-          | intros T3 T4 E2; rewrite E2 in H0; inversion H0;
-              [ rewrite E1 in H2; induction X; discriminate
-              | exact (IHtyping H1 E1 _ _ (sym_eq H5)) ] ]
+        [ intros; discriminate
+        | intros T3 T4 E; exists t; exists T1; trivial
+        | intros T3 T4 E2; rewrite E2 in H0; inversion H0;
+          [ rewrite E1 in H2; induction X; discriminate
+          | exact (IHtyping H1 E1 _ _ (sym_eq H5)) ] ]
       | exists (all T1 T2); trivial ]
-  | exists empty; trivial ].
+    | exists empty; trivial ].
 Qed.
 
 (****)
@@ -1540,33 +1670,33 @@ Qed.
 
 Lemma local_progress :
   forall (t : term) (U : typ),
-  typing empty t U -> value t \/
-  exists c, exists t0, exists t0', red t0 t0' /\ t = ctx_app c t0.
-intros t U H; cut (exists e, e = empty);
-  [ intros (e, E); rewrite <- E in H;
-    induction H;
+    typing empty t U -> value t \/
+                          exists c, exists t0, exists t0', red t0 t0' /\ t = ctx_app c t0.
+  intros t U H; cut (exists e, e = empty);
+    [ intros (e, E); rewrite <- E in H;
+      induction H;
       [ rewrite E in H0; induction x; discriminate
       | simpl; auto
       | right; case (IHtyping1 E); clear IHtyping1;
-          [ intro H2; case (IHtyping2 E); clear IHtyping2;
-              [ intro H3; rewrite E in H; generalize (fun_value H2 H);
-                intros (t', (T1', E1)); rewrite E1; exists c_hole;
-                exists (app (abs T1' t') t2); exists (subst t' 0 t2);
-                split; trivial; apply E_AppAbs; trivial
-              | intros (c, (t0, (t0', (H3, E1)))); exists (c_apparg H2 c);
-                exists t0; exists t0'; rewrite E1; auto ]
-          | intros (c, (t0, (t0', (H3, E1)))); exists (c_appfun c t2);
+        [ intro H2; case (IHtyping2 E); clear IHtyping2;
+          [ intro H3; rewrite E in H; generalize (fun_value H2 H);
+            intros (t', (T1', E1)); rewrite E1; exists c_hole;
+            exists (app (abs T1' t') t2); exists (subst t' 0 t2);
+            split; trivial; apply E_AppAbs; trivial
+          | intros (c, (t0, (t0', (H3, E1)))); exists (c_apparg H2 c);
             exists t0; exists t0'; rewrite E1; auto ]
+        | intros (c, (t0, (t0', (H3, E1)))); exists (c_appfun c t2);
+          exists t0; exists t0'; rewrite E1; auto ]
       | simpl; auto
       | right; case (IHtyping E); clear IHtyping;
-          [ intro H1; rewrite E in H; generalize (typefun_value H1 H);
-            intros (t', (T1', E1)); rewrite E1; exists c_hole;
-            exists (tapp (tabs T1' t') T2); exists (subst_typ t' 0 T2);
-            split; trivial; apply E_TappTabs
-          | intros (c, (t0, (t0', (H3, E1)))); exists (c_typefun c T2);
-            exists t0; exists t0'; rewrite E1; auto ]
+        [ intro H1; rewrite E in H; generalize (typefun_value H1 H);
+          intros (t', (T1', E1)); rewrite E1; exists c_hole;
+          exists (tapp (tabs T1' t') T2); exists (subst_typ t' 0 T2);
+          split; trivial; apply E_TappTabs
+        | intros (c, (t0, (t0', (H3, E1)))); exists (c_typefun c T2);
+          exists t0; exists t0'; rewrite E1; auto ]
       | auto ]
-  | exists empty; trivial ].
+    | exists empty; trivial ].
 Qed.
 
 (****)
@@ -1575,10 +1705,10 @@ Qed.
 
 Theorem progress :
   forall (t : term) (U : typ),
-  typing empty t U -> value t \/ exists t', red t t'.
-intros t U H; generalize (local_progress H);
-intros [H1 | (c, (t0, (t0', (H1, H2))))]; auto;
-right; exists (ctx_app c t0'); rewrite H2; apply E_Ctx; trivial.
+    typing empty t U -> value t \/ exists t', red t t'.
+  intros t U H; generalize (local_progress H);
+    intros [H1 | (c, (t0, (t0', (H1, H2))))]; auto;
+    right; exists (ctx_app c t0'); rewrite H2; apply E_Ctx; trivial.
 Qed.
 
 (****)
@@ -1593,36 +1723,36 @@ Qed.
    typing derivation) as this does not go through...  Instead, our
    proof is by induction on the typing derivation and case on the
    evaluation context.
-*)
+ *)
 
 Lemma context_replacement :
-   forall (e : env) (c : ctx) (t t' : term) (T : typ),
-   (forall (T' : typ), (typing e t T') -> (typing e t' T')) ->
-   typing e (ctx_app c t) T -> typing e (ctx_app c t') T.
-intros e c t t' T H1 H2; cut (exists t'', t'' = ctx_app c t);
-  [ intros (t'', E); rewrite <- E in H2;
-    generalize c E; clear c E; induction H2;
+  forall (e : env) (c : ctx) (t t' : term) (T : typ),
+    (forall (T' : typ), (typing e t T') -> (typing e t' T')) ->
+    typing e (ctx_app c t) T -> typing e (ctx_app c t') T.
+  intros e c t t' T H1 H2; cut (exists t'', t'' = ctx_app c t);
+    [ intros (t'', E); rewrite <- E in H2;
+      generalize c E; clear c E; induction H2;
       [ induction c; try (intros; discriminate); simpl;
         intros E; apply H1; rewrite <- E; apply T_Var; trivial
       | induction c; try (intros; discriminate); simpl;
         intros E; apply H1; rewrite <- E; apply T_Abs; trivial
       | induction c; try (intros; discriminate); simpl;
-          [ intros E; apply H1; rewrite <- E; exact (T_App H2_ H2_0)
-          | intro E; injection E; clear E; intros E1 E2;
-            rewrite <- E1; apply T_App with (2 := H2_0);
-            apply IHtyping1; trivial
-          | intro E; injection E; clear E; intros E1 E2;
-            rewrite <- E2; apply T_App with (1 := H2_);
-            apply IHtyping2; trivial ]
+        [ intros E; apply H1; rewrite <- E; exact (T_App H2_ H2_0)
+        | intro E; injection E; clear E; intros E1 E2;
+          rewrite <- E1; apply T_App with (2 := H2_0);
+          apply IHtyping1; trivial
+        | intro E; injection E; clear E; intros E1 E2;
+          rewrite <- E2; apply T_App with (1 := H2_);
+          apply IHtyping2; trivial ]
       | induction c; try (intros; discriminate); simpl;
         intros E; apply H1; rewrite <- E; exact (T_Tabs H2)
       | induction c; try (intros; discriminate); simpl;
-          [ intros E; apply H1; rewrite <- E; exact (T_Tapp H2 H)
-          | intro E; injection E; clear E; intros E1 E2;
-            rewrite <- E1; apply T_Tapp with (2 := H);
-            apply IHtyping; trivial ]
+        [ intros E; apply H1; rewrite <- E; exact (T_Tapp H2 H)
+        | intro E; injection E; clear E; intros E1 E2;
+          rewrite <- E1; apply T_Tapp with (2 := H);
+          apply IHtyping; trivial ]
       | intros c E; apply T_Sub with (2 := H); apply IHtyping; trivial ]
-  | exists (ctx_app c t); trivial ].
+    | exists (ctx_app c t); trivial ].
 Qed.
 
 (****)
@@ -1631,9 +1761,9 @@ Qed.
 
 Lemma local_preservation_app :
   forall (e : env) (t12 t2 : term) (T11 U : typ),
-  typing e (app (abs T11 t12) t2) U -> typing e (subst t12 0 t2) U.
-intros e t12 t2 T11 U H; cut (exists t, t = app (abs T11 t12) t2);
-  [ intros (t, E); rewrite <- E in H; induction H; try discriminate;
+    typing e (app (abs T11 t12) t2) U -> typing e (subst t12 0 t2) U.
+  intros e t12 t2 T11 U H; cut (exists t, t = app (abs T11 t12) t2);
+    [ intros (t, E); rewrite <- E in H; induction H; try discriminate;
       [ injection E; clear E; intros E1 E2; rewrite E2 in H;
         assert (H6 := proj1 (typing_wf H));
         assert (H7 := proj2 (proj2 (typing_wf H)));
@@ -1642,14 +1772,14 @@ intros e t12 t2 T11 U H; cut (exists t, t = app (abs T11 t12) t2);
         apply (subst_preserves_typing (x := 0) (u := t2) (W := T11) H5);
         trivial; simpl; rewrite <- E1; exact (T_Sub H0 H2)
       | apply T_Sub with (2 := H0); auto ]
-  | exists (app (abs T11 t12) t2); trivial ].
+    | exists (app (abs T11 t12) t2); trivial ].
 Qed.
 
 Lemma local_preservation_tapp :
   forall (e : env) (t12 : term) (T11 T2 U : typ),
-  typing e (tapp (tabs T11 t12) T2) U -> typing e (subst_typ t12 0 T2) U.
-intros e t12 T11 T2 U H; cut (exists t, t = tapp (tabs T11 t12) T2);
-  [ intros (t, E); rewrite <- E in H; induction H; try discriminate;
+    typing e (tapp (tabs T11 t12) T2) U -> typing e (subst_typ t12 0 T2) U.
+  intros e t12 T11 T2 U H; cut (exists t, t = tapp (tabs T11 t12) T2);
+    [ intros (t, E); rewrite <- E in H; induction H; try discriminate;
       [ injection E; clear E; intros E1 E2; rewrite E2 in H;
         assert (H7 := proj1 (typing_wf H));
         assert (H8 := proj2 (proj2 (typing_wf H)));
@@ -1657,7 +1787,7 @@ intros e t12 T11 T2 U H; cut (exists t, t = tapp (tabs T11 t12) T2);
         intros (H2, (T3, (H4, H5))); assert (H6 := T_Sub H5 H4);
         rewrite <- E1; exact (subst_typ_preserves_typing H6 H0)
       | apply T_Sub with (2 := H0); auto ]
-  | exists (tapp (tabs T11 t12) T2); trivial ].
+    | exists (tapp (tabs T11 t12) T2); trivial ].
 Qed.
 
 (****)
@@ -1666,11 +1796,11 @@ Qed.
 
 Theorem preservation :
   forall (e : env) (t t' : term) (U : typ),
-  typing e t U -> red t t' -> typing e t' U.
-intros e t t' U H1 H2; generalize U H1; clear U H1; induction H2; intros U H1;
-  [ exact (local_preservation_app H1)
-  | exact (local_preservation_tapp H1)
-  | exact (context_replacement IHred H1) ].
+    typing e t U -> red t t' -> typing e t' U.
+  intros e t t' U H1 H2; generalize U H1; clear U H1; induction H2; intros U H1;
+    [ exact (local_preservation_app H1)
+    | exact (local_preservation_tapp H1)
+    | exact (context_replacement IHred H1) ].
 Qed.
 
 
@@ -1680,54 +1810,54 @@ Qed.
 
 
 Inductive red' : term -> term -> Prop :=
-  | appabs :
-      forall (t11 : typ) (t12 t2 : term),
-      value t2 -> red' (app (abs t11 t12) t2) (subst t12 0 t2)
-  | tapptabs :
-      forall (t11 t2 : typ) (t12 : term),
-      red' (tapp (tabs t11 t12) t2) (subst_typ t12 0 t2)
-  | appfun :
-      forall t1 t1' t2 : term, red' t1 t1' -> red' (app t1 t2) (app t1' t2)
-  | apparg :
-      forall t1 t2 t2' : term,
-      value t1 -> red' t2 t2' -> red' (app t1 t2) (app t1 t2')
-  | typefun :
-      forall (t1 t1' : term) (t2 : typ),
-      red' t1 t1' -> red' (tapp t1 t2) (tapp t1' t2).
+| appabs :
+  forall (t11 : typ) (t12 t2 : term),
+    value t2 -> red' (app (abs t11 t12) t2) (subst t12 0 t2)
+| tapptabs :
+  forall (t11 t2 : typ) (t12 : term),
+    red' (tapp (tabs t11 t12) t2) (subst_typ t12 0 t2)
+| appfun :
+  forall t1 t1' t2 : term, red' t1 t1' -> red' (app t1 t2) (app t1' t2)
+| apparg :
+  forall t1 t2 t2' : term,
+    value t1 -> red' t2 t2' -> red' (app t1 t2) (app t1 t2')
+| typefun :
+  forall (t1 t1' : term) (t2 : typ),
+    red' t1 t1' -> red' (tapp t1 t2) (tapp t1' t2).
 
 Theorem progress' :
   forall (t : term) (U : typ),
-  typing empty t U -> value t \/ exists t', red' t t'.
-intros t U H; cut (exists e, e = empty);
-  [ intros (e, E); rewrite <- E in H;
-    induction H;
+    typing empty t U -> value t \/ exists t', red' t t'.
+  intros t U H; cut (exists e, e = empty);
+    [ intros (e, E); rewrite <- E in H;
+      induction H;
       [ rewrite E in H0; induction x; discriminate
       | simpl; auto
       | right; case (IHtyping1 E);
-          [ intro H2; case (IHtyping2 E);
-              [ intro H3; rewrite E in H; generalize (fun_value H2 H);
-                intros (t', (T1', E1)); rewrite E1; exists (subst t' 0 t2);
-                apply appabs; trivial
-              | intros (t2', H3); exists (app t1 t2'); apply apparg; trivial ]
-          | intros (t1', H2); exists (app t1' t2); apply appfun; trivial ]
+        [ intro H2; case (IHtyping2 E);
+          [ intro H3; rewrite E in H; generalize (fun_value H2 H);
+            intros (t', (T1', E1)); rewrite E1; exists (subst t' 0 t2);
+            apply appabs; trivial
+          | intros (t2', H3); exists (app t1 t2'); apply apparg; trivial ]
+        | intros (t1', H2); exists (app t1' t2); apply appfun; trivial ]
       | simpl; auto
       | right; case (IHtyping E);
-          [ intro H1; rewrite E in H; generalize (typefun_value H1 H);
-            intros (t', (T1', E1)); rewrite E1; exists (subst_typ t' 0 T2);
-            apply tapptabs; trivial
-          | intros (t1', H1); exists (tapp t1' T2); apply typefun; trivial ]
+        [ intro H1; rewrite E in H; generalize (typefun_value H1 H);
+          intros (t', (T1', E1)); rewrite E1; exists (subst_typ t' 0 T2);
+          apply tapptabs; trivial
+        | intros (t1', H1); exists (tapp t1' T2); apply typefun; trivial ]
       | auto ]
-  | exists empty; trivial ].
+    | exists empty; trivial ].
 Qed.
 
 Theorem preservation' :
   forall (e : env) (t t' : term) (U : typ),
-  typing e t U -> red' t t' -> typing e t' U.
-intros e t t' U H1; generalize t'; clear t'; induction H1;
-  [ intros t' H1; inversion_clear H1
-  | intros t' H2; inversion_clear H2
-  | intros t' H2; generalize H1_ IHtyping1; clear H1_ IHtyping1;
-    inversion_clear H2;
+    typing e t U -> red' t t' -> typing e t' U.
+  intros e t t' U H1; generalize t'; clear t'; induction H1;
+    [ intros t' H1; inversion_clear H1
+    | intros t' H2; inversion_clear H2
+    | intros t' H2; generalize H1_ IHtyping1; clear H1_ IHtyping1;
+      inversion_clear H2;
       [ intros H1 IHtyping1;
         assert (H6 := proj1 (typing_wf H1));
         assert (H7 := proj2 (proj2 (typing_wf H1)));
@@ -1737,14 +1867,14 @@ intros e t t' U H1; generalize t'; clear t'; induction H1;
         trivial; simpl; exact (T_Sub H1_0 H2)
       | intros H1 IHtyping1; apply T_App with (1 := IHtyping1 _ H); trivial
       | intros H2 IHtyping1; apply T_App with (2 := IHtyping2 _ H0); trivial ]
-  | intros t' H2; inversion_clear H2
-  | intros t' H2; generalize H1 IHtyping; clear H1 IHtyping;
-    inversion_clear H2; intros H1 IHtyping;
+    | intros t' H2; inversion_clear H2
+    | intros t' H2; generalize H1 IHtyping; clear H1 IHtyping;
+      inversion_clear H2; intros H1 IHtyping;
       [ assert (H7 := proj1 (typing_wf H1));
         assert (H8 := proj2 (proj2 (typing_wf H1)));
         generalize (t_tabs_inversion H1 (sub_reflexivity H7 H8));
         intros (H2, (T3, (H4, H5))); assert (H6 := T_Sub H5 H4);
         exact (subst_typ_preserves_typing H6 H)
       | apply T_Tapp with (1 := IHtyping _ H0); trivial ]
-  | intros t' H2; eapply T_Sub; auto ].
+    | intros t' H2; eapply T_Sub; auto ].
 Qed.
